
          %%%%% ~~~~~~~~~~~~~~~~~~~~ %%%%%

\section{With-replacement sampling}
\setcounter{theorem}{0}
\setcounter{equation}{0}

%\cite{vanDerVaart1996}
%\cite{Kosorok2008}

%\renewcommand{\theenumi}{\alph{enumi}}
%\renewcommand{\labelenumi}{\textnormal{(\theenumi)}$\;\;$}
\renewcommand{\theenumi}{\roman{enumi}}
\renewcommand{\labelenumi}{\textnormal{(\theenumi)}$\;\;$}

          %%%%% ~~~~~~~~~~~~~~~~~~~~ %%%%%

\begin{theorem}
\mbox{}\vskip 0.2cm
\noindent
Suppose:
\begin{itemize}
\item
	$U = \{1,2,\ldots,N\}$,
	\;and\;
	$p : U \longrightarrow (0,1]$ \;satisfies\; $\underset{u \in U}{\sum}\,p(u) = 1$.
	\vskip 0.1cm
	Then, $p$ induces a probability space structure on $U$.
	We will use the abuse of notation $(U,p)$ to denote the resulting probability space.
\item
	$y : U \longrightarrow \Re$, \;and\; $t_{y} \,:= \underset{u \in U}{\sum}\,y(u)$.
\item
	Let $Z : (U,p) \longrightarrow \Re$ be the random variable by\;
	$Z(u) \,:=\, \dfrac{y(u)}{p(u)}$.
\item
	$n \in \N$, \;and\; $Z_{1}, Z_{2}, \ldots, Z_{n}$ are I.I.D. copies of $Z$.
\end{itemize}
Then,
\begin{enumerate}
\item
	The expected value and variance of $Z$ are given respectively by:
	\begin{equation*}
	E\!\left[\;Z\;\right] \;=\; t_{y}
	\quad\quad\textnormal{and}\quad\quad
	\Var\!\left[\;Z\;\right] \;=\; \underset{u \in U}{\sum}\;\; p(u)\cdot\left(\,\dfrac{y(u)}{p(u)}\,-\,t_{y}\,\right)^{2}
	\end{equation*}
\item
	$\overline{Z}_{n}\,:=\,\dfrac{1}{n}\;\overset{n}{\underset{i=1}{\sum}}\,Z_{i}$
	is an unbiased estimator of $t_{y}$;
	in other words,
	\begin{equation*}
	E\!\left[\;\overline{Z}_{n}\;\right]
	\;\; = \;\;
		E\!\left[\;\dfrac{1}{n}\;\overset{n}{\underset{i=1}{\sum}}\,Z_{i}\;\right]
	\;\; = \;\;
		t_{y}
	\end{equation*}
\item
	The variance of \;$\overline{Z}_{n}$ is given by
	\begin{equation*}
	\Var\!\left[\;\overline{Z}_{n}\;\right]
	\;\; = \;\;
		\Var\!\left[\;\dfrac{1}{n}\;\overset{n}{\underset{i=1}{\sum}}\,Z_{i}\;\right]
	\;\; = \;\;
		\dfrac{1}{n}\cdot\Var\!\left[\;Z\;\right]
	\;\; = \;\;
		\dfrac{1}{n} \cdot \underset{u \in U}{\sum}\;\,p(u)\cdot\left(\,\dfrac{y(u)}{p(u)}\,-\,t_{y}\,\right)^{2}
	\end{equation*}
\item
	$\dfrac{1}{n-1}\;\overset{n}{\underset{i=1}{\sum}}\left(\,Z_{i} \,-\, \overline{Z}_{n}\,\right)^{2}$\;
	is an unbiased estimator of \,$\Var\!\left[\;Z\;\right]$; in other words,	
	\begin{equation*}
	E\!\left[\;\,\dfrac{1}{n-1}\;\overset{n}{\underset{i=1}{\sum}}\left(\,Z_{i} \,-\, \overline{Z}_{n}\,\right)^{2}\;\right]
	\;\; = \;\;
		\Var\!\left[\;Z\;\right]
	\end{equation*}
\item
	$\dfrac{1}{n}\left(\,\dfrac{1}{n-1}\;\overset{n}{\underset{i=1}{\sum}}\left(\,Z_{i} \,-\, \overline{Z}_{n}\,\right)^{2}\,\right)$\;
	is an unbiased estimator of \,$\Var\!\left[\;\overline{Z}_{n}\;\right]$; in other words,	
	\begin{equation*}
	E\!\left[\;\,\dfrac{1}{n}\left(\,\dfrac{1}{n-1}\;\overset{n}{\underset{i=1}{\sum}}\left(\,Z_{i} \,-\, \overline{Z}_{n}\,\right)^{2}\,\right)\;\right]
	\;\; = \;\;
		\Var\!\left[\;\overline{Z}_{n}\;\right]
	\;\; = \;\;
		\dfrac{1}{n}\cdot\Var\!\left[\;Z\;\right]
	\end{equation*}
\item
	For each $u \in U$, the probability \;$\pi_{u} \in (0,1]$\, of selecting \;$u \in U$\,
	in an independent with-replacement random sample from \,$(U,p)$\, satisfies:
	\begin{equation*}
	\pi_{u}
	\;\; = \;\;
		n \cdot p(u)
		\; + \;
		O\!\left(\,\overset{{\color{white}-}}{p}(u)^{2}\,\right)
	\end{equation*}
\end{enumerate}
\end{theorem}
\proof
\begin{enumerate}
\item
	Observe that
	\begin{eqnarray*}
	E\!\left[\;Z\;\right]
	&=&
		\underset{u \in U}{\sum}\;\; p(u) \cdot Z(u)
	\;\; = \;\;
		\underset{u \in U}{\sum}\;\; p(u) \cdot \dfrac{y(u)}{p(u)}
	\;\; = \;\;
		\underset{u \in U}{\sum}\;\; y(u)
	\;\; = \;\;
		t_{y}
	\end{eqnarray*}
	Secondly, since \;$E\!\left[\;Z\;\right] \,=\, t_{y}$,\; we have
	\begin{eqnarray*}
	\Var\!\left[\;Z\;\right]
	&=&
		E\!\left[\;(Z\,-\,t_{y})^{2}\;\right]	
	\;\; = \;\;
		\underset{u \in U}{\sum}\;\, p(u)\cdot\left(\overset{{\color{white}.}}{Z}(u)\,-\,t_{y}\,\right)^{2}
	\;\; = \;\;
		\underset{u \in U}{\sum}\;\, p(u)\cdot\left(\,\dfrac{y(u)}{p(u)}\,-\,t_{y}\,\right)^{2}
	\end{eqnarray*}
\item
	Observe that
	\begin{eqnarray*}
	E\!\left[\;\dfrac{1}{n}\;\overset{n}{\underset{i=1}{\sum}}\,Z_{i}\;\right]
	&=&
		\dfrac{1}{n}\;\overset{n}{\underset{i=1}{\sum}}\;E\!\left[\;Z_{i}\;\right]
	\;\; = \;\;
		\dfrac{1}{n}\;\overset{n}{\underset{i=1}{\sum}}\;E\!\left[\;Z\;\right]
	\;\; = \;\;
		E\!\left[\;Z\;\right]
	\;\; = \;\;
		t_{y}\,,
	\end{eqnarray*}
	as desired.
\item
	Since \;$E\!\left[\;\dfrac{1}{n}\;\overset{n}{\underset{i=1}{\sum}}\,Z_{i}\;\right]$ $=$\, $t_{y}$,\;
	and \;$Z_{1}, \ldots, Z_{n}$\; are independent, we have:
	\begin{eqnarray*}
	\Var\!\left[\;\dfrac{1}{n}\;\overset{n}{\underset{i=1}{\sum}}\,Z_{i}\;\right]
	&=&
		\dfrac{1}{n^{2}}\;\overset{n}{\underset{i=1}{\sum}}\;\Var\!\left[\;Z_{i}\;\right]
	\;\; = \;\;
		\dfrac{1}{n^{2}}\;\overset{n}{\underset{i=1}{\sum}}\;\Var\!\left[\;Z\;\right]
	\;\; = \;\;
		\dfrac{1}{n}\cdot\Var\!\left[\;Z\;\right]
	\\
	&=&
		\dfrac{1}{n}\cdot
		\underset{u \in U}{\sum}\;\, p(u)\cdot\left(\,\dfrac{y(u)}{p(u)}\,-\,t_{y}\,\right)^{2}\,,
	\end{eqnarray*}
	as desired.
\item
	In order to see that
	\begin{eqnarray*}
	E\!\left[\;\,\dfrac{1}{n-1}\;\overset{n}{\underset{i=1}{\sum}}\left(\,Z_{i} \,-\, \overline{Z}_{n}\,\right)^{2}\;\right]
	\;\; = \;\;
		\Var\!\left[\;Z\;\right],
	\end{eqnarray*}
	observe first that
	\begin{eqnarray*}
	E\!\left[\;\left(\,Z_{i} \,-\, \overline{Z}_{n}\,\right)^{2}\;\right]
	& = &
		E\!\left[\;Z_{i}^{2} \,-\, 2\,Z_{i}\,\overline{Z}_{n} \,+\, \overline{Z}_{n}^{2}\;\right]
	\;\; = \;\;
		E\!\left[\;Z_{i}^{2}\;\right]
		\,-\, 2 \cdot E\!\left[\;Z_{i}\cdot\overline{Z}_{n}\;\right]
		\,+\, E\!\left[\;\overline{Z}_{n}^{2}\;\right]
	\\
	& = &
		E\!\left[\;Z^{2}\;\right]
		\,-\, 2 \cdot E\!\left[\;Z_{i}\cdot\left(\dfrac{1}{n}\;\overset{n}{\underset{k=1}{\sum}}\;Z_{k}\right)\;\right]
		\,+\, \Var\!\left[\;\overline{Z}_{n}\;\right] + E\!\left[\;\overline{Z}_{n}\;\right]^{2}
	\\
	& = &
		\Var\!\left[\;Z\;\right] + E\!\left[\;Z\;\right]^{2}
		\,-\, \dfrac{2}{n} \cdot \overset{n}{\underset{k=1}{\sum}} \; E\!\left[\;Z_{i} \cdot Z_{k}\;\right]
		\,+\, \dfrac{1}{n}\cdot\Var\!\left[\;Z\;\right] + E\!\left[\;\overline{Z}\;\right]^{2}
	\\
	& = &
		\left(1+\dfrac{1}{n}\right)\cdot\Var\!\left[\;Z\;\right] + 2 \cdot E\!\left[\;Z\;\right]^{2}
		\,-\, \dfrac{2}{n} \cdot \left(
			E\!\left[\;Z_{i}^{2}\;\right] + \underset{k \neq i}{\sum} \; E\!\left[\;Z_{i} \cdot Z_{k}\;\right]
			\right)
	\\
	& = &
		\left(1+\dfrac{1}{n}\right)\cdot\Var\!\left[\;Z\;\right] + 2 \cdot E\!\left[\;Z\;\right]^{2}
		\,-\, \dfrac{2}{n} \cdot \left(
			\Var\!\left[\;Z\;\right] + E\!\left[\;Z\;\right]^{2} + (n-1)\cdot E\!\left[\;Z\;\right]^{2}
			\right)
	\\
	& = &
		\left(1+\dfrac{1}{n}\right)\cdot\Var\!\left[\;Z\;\right] + 2 \cdot E\!\left[\;Z\;\right]^{2}
		\,-\, \dfrac{2}{n} \cdot \left(
			\Var\!\left[\;Z\;\right] + n\cdot E\!\left[\;Z\;\right]^{2}
			\right)
	\\
	& = &
		\left(1-\dfrac{1}{n}\right)\cdot\Var\!\left[\;Z\;\right]
	\;\; = \;\;
		\left(\dfrac{n-1}{n}\right)\cdot\Var\!\left[\;Z\;\right]
	\end{eqnarray*}
	Consequently,
	\begin{eqnarray*}
	E\!\left[\;\,\dfrac{1}{n-1}\;\overset{n}{\underset{i=1}{\sum}}\left(\,Z_{i} \,-\, \overline{Z}_{n}\,\right)^{2}\;\right]
	&=&
		\dfrac{1}{n-1}\cdot
		\overset{n}{\underset{i=1}{\sum}}\;E\!\left[\;\left(\,Z_{i} \,-\, \overline{Z}_{n}\,\right)^{2}\;\right]
	\;\; = \;\;
		\dfrac{1}{n-1}\cdot
		\overset{n}{\underset{i=1}{\sum}}\,\left(\dfrac{n-1}{n}\right)\cdot\Var\!\left[\;Z\;\right]
	\\
	&=&
		\dfrac{1}{n-1} \cdot n \cdot \left(\dfrac{n-1}{n}\right)\cdot\Var\!\left[\;Z\;\right]
	\;\; = \;\;
		\Var\!\left[\;Z\;\right],
	\end{eqnarray*}
	as desired.
\item
	Immediate by the preceding result.
\item
	\begin{eqnarray*}
	\pi_{u}
	& = &
		1 - \left(\,1 - \overset{{\color{white}-}}{p}(u)\,\right)^{n}
	\;\; = \;\;
		1 \; - \;
			\overset{n}{\underset{i=0}{\sum}}\,
			\left(\!\begin{array}{c}n \\ i\end{array}\!\right)
			\left(\,1\,\right)^{n-i}\cdot\left(\,-\,\overset{{\color{white}-}}{p}(u)\,\right)^{i}
	\;\; = \;\;
		1 \; - \;
			\overset{n}{\underset{i=0}{\sum}}\,
			\left(\!\begin{array}{c}n \\ i\end{array}\!\right)
			\left(\,-1\,\right)^{i} \cdot p(u)^{i}
	\\
	& = &
		1 \; - \; 1 \; + \; n\cdot p(u) \; + \;
			\overset{n}{\underset{i=2}{\sum}}\,
			\left(\!\begin{array}{c}n \\ i\end{array}\!\right)
			\left(\,-1\,\right)^{i} \cdot p(u)^{i}
	\\
	& = &
		n\cdot p(u) \; + \;
			\overset{n}{\underset{i=2}{\sum}}\,
			\left(\!\begin{array}{c}n \\ i\end{array}\!\right)
			\left(\,-1\,\right)^{i} \cdot p(u)^{i}
	\end{eqnarray*}
\end{enumerate}
This completes the proof of the Theorem.
\qed

          %%%%% ~~~~~~~~~~~~~~~~~~~~ %%%%%

%\renewcommand{\theenumi}{\alph{enumi}}
%\renewcommand{\labelenumi}{\textnormal{(\theenumi)}$\;\;$}
\renewcommand{\theenumi}{\roman{enumi}}
\renewcommand{\labelenumi}{\textnormal{(\theenumi)}$\;\;$}

          %%%%% ~~~~~~~~~~~~~~~~~~~~ %%%%%
