
\noindent
\textbf{Exercise 2.26(a)}

Recall that:
\begin{equation*}
h(t)
\; := \;
\lim_{h \rightarrow 0}
\dfrac{P(t \leq T \leq t + h \,\vert\, t \leq T )}{h},
\quad\quad
F(t) \; = \; P(T < t), 
\quad\quad
f(t) \; = \; F^{\prime}(t),
\quad\quad
S(t) = 1 - F(t)
\end{equation*}
We want to prove:
\begin{equation*}
h(t)
\; = \;
\dfrac{f(t)}{S(t)}.
\end{equation*}
\proof
\begin{eqnarray*}
    P(t \leq T \leq t + h \,\vert\, t \leq T)
&=&       \dfrac{P(t \leq T \leq t + h \,\cap\, t \leq T)}{P(t \leq T)}
\;\;=\;\; \dfrac{P(t \leq T \leq t + h)}{P(t \leq T)}
\;\;=\;\; \dfrac{P(T \leq t + h) - P(T \leq t)}{P(t \leq T)} \\
&=&       \dfrac{F(t+h)-F(t)}{1 - F(t)}
\end{eqnarray*}
Hence,
\begin{eqnarray*}
    \dfrac{P(t \leq T \leq t + h \,\vert\, t \leq T)}{h}
&=& \dfrac{1}{1-F(t)}\cdot\dfrac{F(t + h) - F(t)}{h}
\end{eqnarray*}
Hence,
\begin{eqnarray*}
h(t)
&=&       \lim_{h \rightarrow 0} \dfrac{P(t \leq T \leq t + h \,\vert\, t \leq T )}{h} 
\;\;=\;\; \dfrac{1}{1-F(t)}\cdot\lim_{h\rightarrow 0}\dfrac{F(t + h) - F(t)}{h}
\;\;=\;\; \dfrac{1}{1-F(t)}\cdot F^{\prime}(t)
\;\;=\;\; \dfrac{f(t)}{S(t)}
\end{eqnarray*}
\qed

%%%%%%%%%%%%%%%%%%%%%%%%%%%%%%%%%%%%%%%%%%%%%%%%%%%%%%%%%%%%%%%%%%%%%%%%%%%%%%%%%%%%%%%%%%%%%%%%%%%%
%\newpage
\noindent
\textbf{Exercise 2.26(b)}

