
          %%%%% ~~~~~~~~~~~~~~~~~~~~ %%%%%

\section{Derivatives of $E\!\left[\,\left.\log\,L\,\right\vert\,\mathcal{D}\,\right]$ with respect to $\mu_{1 \vert gy}$}
\setcounter{theorem}{0}
\setcounter{equation}{0}

\renewcommand{\theenumi}{\roman{enumi}}
\renewcommand{\labelenumi}{\textnormal{(\theenumi)}$\;\;$}

\begin{eqnarray*}
\log\,L
	&=&
	\log\,P\!\left(\;
		\overset{n}{\underset{i=1}{\bigcap}}\;
		\left\{
			Y^{(i)}=c_{i},X^{(i)}=x_{i},\widetilde{Y}^{(i)}=y_{i},K^{(i)}=k_{i}
		\right\}
	\;\right)
\\
&=&
	{\color{white}+} \;\;
	\overset{C}{\underset{c=1}{\sum}}\;\;
	\overset{G}{\underset{g=1}{\sum}}\;\;
	\overset{C}{\underset{y=1}{\sum}}\;
	\left(\overset{n}{\underset{i=1}{\sum}}\;W^{(i)}_{c \vert gy{\color{red}0}}\right)
	\cdot
	\left(\,
		\log\left(\pi_{c \vert g}\,\mu_{0 \vert gy} + \delta_{cy}\,\mu_{1\vert gy}\right)
		\,\overset{{\color{white}.}}{+}\,
		\log\,\nu_{gy}
		\,\overset{{\color{white}.}}{+}\,
		\log\,\omega_{0}
	\,\right)
\\
&&
	+ \;\;
	\overset{C}{\underset{c=1}{\sum}}\;\;
	\overset{G}{\underset{g=1}{\sum}}\;\;
	\overset{C}{\underset{y=1}{\sum}}\;
	\left(\overset{n}{\underset{i=1}{\sum}}\;W^{(i)}_{c \vert gy{\color{red}1}}\right)
	\cdot
	\left(\,
		\log\,\pi_{c \vert g}
		\,\overset{{\color{white}.}}{+}\,
		\log\,\mu_{0\vert gy}
		\,\overset{{\color{white}.}}{+}\,
		\log\,\nu_{gy}
		\,\overset{{\color{white}.}}{+}\,
		\log\,\omega_{1}
	\,\right)
\\
&&
	+ \;\;
	\overset{C}{\underset{y=1}{\sum}}\;\;
	\overset{G}{\underset{g=1}{\sum}}\;
	\left(\overset{n}{\underset{i=1}{\sum}}\;W^{(i)}_{y \vert gy{\color{red}2}}\right)
	\cdot
	\left(\,
		\log\,\mu_{1 \vert gy}
		\,\overset{{\color{white}.}}{+}\,
		\log\,\nu_{gy}
		\,\overset{{\color{white}.}}{+}\,
		\log\,\omega_{1}
	\,\right)
\end{eqnarray*}

\begin{eqnarray*}
E\!\left[\,\left.\log\,L\;\right\vert\;\mathcal{D}\,\right]
&=& T_{0} \;+\; T_{1} \;+\; T_{2}
\\
T_{0}
&:=&
	\overset{C}{\underset{c=1}{\sum}}\;\;
	\overset{G}{\underset{g=1}{\sum}}\;\;
	\overset{C}{\underset{y=1}{\sum}}\;\;
	E_{c \vert gy{\color{red}0}}
	\cdot
	\left(\,
		\log\left(\pi_{c \vert g}\,\mu_{0 \vert gy} + \delta_{cy}\,\mu_{1\vert gy}\right)
		\,\overset{{\color{white}.}}{+}\,
		\log\,\nu_{gy}
		\,\overset{{\color{white}.}}{+}\,
		\log\,\omega_{0}
	\,\right)
\\
T_{1}
&:=&
	\overset{C}{\underset{c=1}{\sum}}\;\;
	\overset{G}{\underset{g=1}{\sum}}\;\;
	\overset{C}{\underset{y=1}{\sum}}\;\;
	E_{c \vert gy{\color{red}1}}
	\cdot
	\left(\,
		\log\,\pi_{c \vert g}
		\,\overset{{\color{white}.}}{+}\,
		\log\,\mu_{0\vert gy}
		\,\overset{{\color{white}.}}{+}\,
		\log\,\nu_{gy}
		\,\overset{{\color{white}.}}{+}\,
		\log\,\omega_{1}
	\,\right)
\\
T_{2}
&:=&
	\overset{C}{\underset{y=1}{\sum}}\;\;
	\overset{G}{\underset{g=1}{\sum}}\;\;
	E_{y \vert gy{\color{red}2}}
	\cdot
	\left(\,
		\log\,\mu_{1 \vert gy}
		\,\overset{{\color{white}.}}{+}\,
		\log\,\nu_{gy}
		\,\overset{{\color{white}.}}{+}\,
		\log\,\omega_{1}
	\,\right)
\end{eqnarray*}

\begin{eqnarray*}
T_{0}
&:=&
	\overset{C}{\underset{c=1}{\sum}}\;\;
	\overset{G}{\underset{g=1}{\sum}}\;\;
	\overset{C}{\underset{y=1}{\sum}}\;\;
	E_{c \vert gy{\color{red}0}}
	\cdot
	\left(\,
		\log\left(\pi_{c \vert g}\,\mu_{0 \vert gy} + \delta_{cy}\,\mu_{1\vert gy}\right)
		\,\overset{{\color{white}.}}{+}\,
		\log\,\nu_{gy}
		\,\overset{{\color{white}.}}{+}\,
		\log\,\omega_{0}
	\,\right)
\\
&=&
	\overset{G}{\underset{g=1}{\sum}}\;\;
	\overset{C}{\underset{y=1}{\sum}}\;\;
	\overset{C}{\underset{c=1}{\sum}}\;\;
	E_{c \vert gy{\color{red}0}}
	\cdot
	\log\left(\pi_{c \vert g}\,(1-\mu_{1 \vert gy}) \overset{{\color{white}.}}{+} \delta_{cy}\,\mu_{1\vert gy}\right)
	\;\; + \;\;
	\overset{G}{\underset{g=1}{\sum}}\;\;
	\overset{C}{\underset{y=1}{\sum}}\;\;
	\overset{C}{\underset{c=1}{\sum}}\;\;
	E_{c \vert gy{\color{red}0}}
	\cdot
	\left(\,
		\log\,\nu_{gy}
		\,\overset{{\color{white}.}}{+}\,
		\log\,\omega_{0}
	\,\right)	
\\
&=&
	\overset{G}{\underset{g=1}{\sum}}\;\;
	\overset{C}{\underset{y=1}{\sum}}\;\;
	\overset{C}{\underset{c=1}{\sum}}\;\;
	E_{c \vert gy{\color{red}0}}
	\cdot
	\log\left(\pi_{c \vert g} \overset{{\color{white}.}}{+} (\delta_{cy}-\pi_{c \vert g})\,\mu_{1\vert gy}\right)
	\;\; + \;\;
	\overset{G}{\underset{g=1}{\sum}}\;\;
	\overset{C}{\underset{y=1}{\sum}}\;\;
	\overset{C}{\underset{c=1}{\sum}}\;\;
	E_{c \vert gy{\color{red}0}}
	\cdot
	\left(\,
		\log\,\nu_{gy}
		\,\overset{{\color{white}.}}{+}\,
		\log\,\omega_{0}
	\,\right)	
\end{eqnarray*}

\begin{eqnarray*}
\dfrac{\partial\,T_{0}}{\partial\,\mu_{1 \vert gy}}
&=&
	\overset{C}{\underset{c=1}{\sum}}\;\;
	\dfrac{E_{c \vert gy{\color{red}0}} \cdot (\delta_{cy}-\pi_{c \vert g})}{
		\pi_{c \vert g} + (\delta_{cy}-\pi_{c \vert g})\,\mu_{1\vert gy}
		}
\;\;=\;\;
	\dfrac{E_{y \vert gy{\color{red}0}} \cdot (\delta_{yy}-\pi_{y \vert g})}{
		\pi_{y \vert g} + (\delta_{yy}-\pi_{y \vert g})\,\mu_{1\vert gy}
		}
	\; + \;
	\underset{c\neq y}{\overset{C}{\underset{c=1}{\sum}}}\;\;
	\dfrac{E_{c \vert gy{\color{red}0}} \cdot (\delta_{cy}-\pi_{c \vert g})}{
		\pi_{c \vert g} + (\delta_{cy}-\pi_{c \vert g})\,\mu_{1\vert gy}
		}
\\
&=&
	\dfrac{E_{y \vert gy{\color{red}0}} \cdot (1-\pi_{y \vert g})}{
		\pi_{y \vert g} + (1-\pi_{y \vert g})\,\mu_{1\vert gy}
		}
	\; + \;
	\underset{c\neq y}{\overset{C}{\underset{c=1}{\sum}}}\;\;
	\dfrac{E_{c \vert gy{\color{red}0}} \cdot (-\pi_{c \vert g})}{
		\pi_{c \vert g} + (-\pi_{c \vert g})\,\mu_{1\vert gy}
		}
\;\;=\;\;
	\dfrac{E_{y \vert gy{\color{red}0}} \cdot (1-\pi_{y \vert g})}{
		\pi_{y \vert g} + (1-\pi_{y \vert g})\,\mu_{1\vert gy}
		}
	\; - \;
	\underset{c\neq y}{\overset{C}{\underset{c=1}{\sum}}}\;\;
	\dfrac{E_{c \vert gy{\color{red}0}}}{1 - \mu_{1\vert gy}}
\\
&=&
	\dfrac{E_{y \vert gy{\color{red}0}} \cdot (1-\pi_{y \vert g})}{
		\pi_{y \vert g} + (1-\pi_{y \vert g})\,\mu_{1\vert gy}
		}
	\; - \;
	\dfrac{1}{1 - \mu_{1\vert gy}}
	\cdot
	\underset{c\neq y}{\overset{C}{\underset{c=1}{\sum}}}\; E_{c \vert gy{\color{red}0}}
\\
&=&
	\dfrac{E_{y \vert gy{\color{red}0}} \cdot (1-\pi_{y \vert g})}{
		\pi_{y \vert g} + (1-\pi_{y \vert g})\,\mu_{1\vert gy}
		}
	\; - \;
	\dfrac{1}{1 - \mu_{1\vert gy}}
	\cdot
	\left(-\,E_{y \vert gy{\color{red}0}} + \overset{C}{\underset{c=1}{\sum}}\; E_{c \vert gy{\color{red}0}}\right)
\\
&=&
	\dfrac{E_{y \vert gy{\color{red}0}} \cdot (1-\pi_{y \vert g})}{
		\pi_{y \vert g} + (1-\pi_{y \vert g})\,\mu_{1\vert gy}
		}
	\; + \; \dfrac{E_{y \vert gy{\color{red}0}}}{1 - \mu_{1\vert gy}}
	\; - \; \dfrac{1}{1 - \mu_{1\vert gy}} \cdot \overset{C}{\underset{c=1}{\sum}}\; E_{c \vert gy{\color{red}0}}
\\
&=&
	E_{y \vert gy{\color{red}0}} \cdot
	\left(\;
		\dfrac{1-\pi_{y \vert g}}{\pi_{y \vert g} + (1-\pi_{y \vert g})\,\mu_{1\vert gy} }
		\; + \;
		\dfrac{1}{1 - \mu_{1\vert gy}}
	\;\right)
	\; - \; \dfrac{1}{1 - \mu_{1\vert gy}} \cdot \overset{C}{\underset{c=1}{\sum}}\; E_{c \vert gy{\color{red}0}}
\end{eqnarray*}

\begin{eqnarray*}
T_{1}
&:=&
	\overset{C}{\underset{c=1}{\sum}}\;\;
	\overset{G}{\underset{g=1}{\sum}}\;\;
	\overset{C}{\underset{y=1}{\sum}}\;\;
	E_{c \vert gy{\color{red}1}}
	\cdot
	\left(\,
		\log\,\pi_{c \vert g}
		\,\overset{{\color{white}.}}{+}\,
		\log\,\mu_{0\vert gy}
		\,\overset{{\color{white}.}}{+}\,
		\log\,\nu_{gy}
		\,\overset{{\color{white}.}}{+}\,
		\log\,\omega_{1}
	\,\right)
\\
&=&
	\overset{G}{\underset{g=1}{\sum}}\;\;
	\overset{C}{\underset{y=1}{\sum}}\;\;
	\overset{C}{\underset{c=1}{\sum}}\;\;
	E_{c \vert gy{\color{red}1}} \cdot \log\,(1-\mu_{1\vert gy})
	\; + \;
	\overset{G}{\underset{g=1}{\sum}}\;\;
	\overset{C}{\underset{y=1}{\sum}}\;\;
	\overset{C}{\underset{c=1}{\sum}}\;\;
	E_{c \vert gy{\color{red}1}}
	\cdot
	\left(\,
		\log\,\pi_{c \vert g}
		\,\overset{{\color{white}.}}{+}\,
		\log\,\nu_{gy}
		\,\overset{{\color{white}.}}{+}\,
		\log\,\omega_{1}
	\,\right)
\end{eqnarray*}

\begin{eqnarray*}
\dfrac{\partial\,T_{1}}{\partial\,\mu_{1 \vert gy}}
&=&
	\overset{C}{\underset{c=1}{\sum}} \;\; \dfrac{E_{c \vert gy{\color{red}1}}\cdot(-1)}{1-\mu_{1\vert gy}}
	\;\; = \;\;
	\dfrac{-1}{1-\mu_{1\vert gy}} \cdot \overset{C}{\underset{c=1}{\sum}}\; E_{c \vert gy{\color{red}1}}
\end{eqnarray*}

\begin{eqnarray*}
\dfrac{\partial\,T_{2}}{\partial\,\mu_{1 \vert gy}}
&=&
	\dfrac{E_{y \vert gy{\color{red}2}}}{\mu_{1 \vert gy}}
\end{eqnarray*}

\begin{eqnarray*}
\dfrac{\partial\;E\!\left[\,\left.\log\,L\;\right\vert\;\mathcal{D}\,\right]}{\partial\;\mu_{1 \vert gy}}
&=&
	\dfrac{\partial\;T_{0}}{\partial\;\mu_{1 \vert gy}}
	\;+\;
	\dfrac{\partial\;T_{1}}{\partial\;\mu_{1 \vert gy}}
	\;+\;
	\dfrac{\partial\;T_{2}}{\partial\;\mu_{1 \vert gy}}
\\
&=&
	{\color{white}+} \;\;
	E_{y \vert gy{\color{red}0}} \cdot
	\left(\;
		\dfrac{1-\pi_{y \vert g}}{\pi_{y \vert g} + (1-\pi_{y \vert g})\,\mu_{1\vert gy} }
		\; + \;
		\dfrac{1}{1 - \mu_{1\vert gy}}
	\;\right)
	\; - \; \dfrac{1}{1 - \mu_{1\vert gy}} \cdot \overset{C}{\underset{c=1}{\sum}}\; E_{c \vert gy{\color{red}0}}
\\
&&
	+ \;\;
	\dfrac{-1}{1-\mu_{1\vert gy}} \cdot \overset{C}{\underset{c=1}{\sum}}\; E_{c \vert gy{\color{red}1}}
	\; + \;
	\dfrac{E_{y \vert gy{\color{red}2}}}{\mu_{1 \vert gy}}
\\
&=&
	E_{y \vert gy0} \cdot
	\left(\;
		\dfrac{1-\pi_{y \vert g}}{\pi_{y \vert g} + (1-\pi_{y \vert g})\,\mu_{1\vert gy} }
		\; + \;
		\dfrac{1}{1 - \mu_{1\vert gy}}
	\;\right)
	\; - \;
	\dfrac{1}{1-\mu_{1\vert gy}}
	\cdot
	\left(\,
		\overset{C}{\underset{c=1}{\sum}}\;
		\overset{1}{\underset{k=0}{\sum}}\;
		E_{c \vert gyk}
	\right)
	\; + \;
	\dfrac{E_{y \vert gy2}}{\mu_{1 \vert gy}}
\\
&=&
	\dfrac{(1-\pi_{y \vert g}) \cdot E_{y \vert gy0}}{\pi_{y \vert g} + (1-\pi_{y \vert g})\cdot{\color{red}\mu_{1\vert gy}}}
	\; + \;
	\dfrac{1}{1-{\color{red}\mu_{1\vert gy}}}
	\cdot
	\left(\,
		E_{y \vert gy0}
		\;-\;
		\overset{C}{\underset{c=1}{\sum}}\;
		\overset{1}{\underset{k=0}{\sum}}\;
		E_{c \vert gyk}
	\right)
	\; + \;
	\dfrac{E_{y \vert gy2}}{\color{red}\mu_{1 \vert gy}}
\end{eqnarray*}

\begin{eqnarray*}
&&
	\dfrac{\partial\;E\!\left[\,\left.\log\,L\;\right\vert\;\mathcal{D}\,\right]}{\partial\;\mu_{1 \vert gy}} \;=\; 0\,,
	\quad\forall\;\,y\;\in\,\{1,\ldots,C\}
\\
&\Longrightarrow&
	\dfrac{(1-\pi_{y \vert g}) \cdot E_{y \vert gy0}}{\pi_{y \vert g} + (1-\pi_{y \vert g})\cdot{\color{red}\mu_{1\vert gy}}}
	\; + \;
	\dfrac{1}{1-{\color{red}\mu_{1\vert gy}}}
	\cdot
	\left(\,
		E_{y \vert gy0}
		\;-\;
		\overset{C}{\underset{c=1}{\sum}}\;
		\overset{1}{\underset{k=0}{\sum}}\;
		E_{c \vert gyk}
	\right)
	\; + \;
	\dfrac{E_{y \vert gy2}}{\color{red}\mu_{1 \vert gy}}
	\; = \; 0 \,,
	\quad\forall\;\,y\;\in\,\{1,\ldots,C\}	
\end{eqnarray*}

          %%%%% ~~~~~~~~~~~~~~~~~~~~ %%%%%
