
\noindent
\textbf{Exercise 1.1(a)}

Let $X$ be the sum of the two number obtained.

Let $X_{1}$ be the number obtained on Die 1.

Let $X_{2}$ be the number obtained on Die 2.

Thus, $X = X_{1} + X_{2}$, and
\begin{equation*}
E_{x}
=
\{X = x\} = \{X_{1} + X_{2} = x\}
=
\{\; X_{1} = x_{1}, X_{2} = x - x_{1} \;\vert\; 1 \leq x_{1}, x - x_{1} \leq 6 \;\}
\end{equation*}
Now,
\begin{equation*}
1 \leq x - x_{1} \leq 6
\quad\Longleftrightarrow\quad
-1 \geq x_{1} - x \geq -6
\quad\Longleftrightarrow\quad
x-1 \geq x_{1} \geq x-6
\quad\Longleftrightarrow\quad
x-6 \leq x_{1} \leq x-1
\end{equation*}
Hence,
\begin{equation*}
E_{x}
=
\{X = x\} = \{X_{1} + X_{2} = x\}
=
\{\; X_{1} = x_{1}, X_{2} = x - x_{1}
\;\vert\;
\max\{1,x-6\} \leq x_{1} \leq \min\{6,x-1\} 
\;\}
\end{equation*}
\begin{eqnarray*}
P(E_{x})
& = &
\sum_{x_{1}=\max\{1,x-6\}}^{\min\{6,x-1\}}\,P(X_{1}=x_{1},X_{2}=x-x_{1})
\;\; = \;\;
\sum_{x_{1}=\max\{1,x-6\}}^{\min\{6,x-1\}}\,\dfrac{1}{6^{2}} \\
& & \\
& = &
\dfrac{1}{6^{2}}\left( \min\{6,x-1\} - \max\{1,x-6\} + 1 \right)
\end{eqnarray*}
Next, note that
\begin{equation*}
\min\{6,x-1\}
=
\left\{\begin{array}{cl}
x - 1, & \textnormal{if $x$ = 2, 3, \ldots,  6} \\
6,     & \textnormal{if $x$ = 7, 8, \ldots, 12} \\
\end{array}\right.
\quad\textnormal{and}\quad
\max\{1,x-6\}
=
\left\{\begin{array}{cl}
1,     & \textnormal{if $x$ = 2, 3, \ldots,  6} \\
x - 6, & \textnormal{if $x$ = 7, 8, \ldots, 12} \\
\end{array}\right.
\end{equation*}
Hence,
\begin{eqnarray*}
P(E_{x})
& = &
\dfrac{1}{6^{2}}\left( \min\{6,x-1\} - \max\{1,x-6\} + 1 \right) 
\;\; = \;\;
\dfrac{1}{36}\left\{\begin{array}{cl}
(x-1) - 1 + 1  , & \textnormal{if $x$ = 2, 3, \ldots,  6} \\
6 - (x - 6) + 1, & \textnormal{if $x$ = 7, 8, \ldots, 12} \\
\end{array}\right.
\\
& = &
\dfrac{1}{36}\left\{\begin{array}{cl}
 x - 1, & \textnormal{if $x$ = 2, 3, \ldots,  6} \\
13 - x, & \textnormal{if $x$ = 7, 8, \ldots, 12} \\
\end{array}\right.
\end{eqnarray*}
\qed
