
          %%%%% ~~~~~~~~~~~~~~~~~~~~ %%%%%

\section{Exploratory calculations}
\setcounter{theorem}{0}
\setcounter{equation}{0}

\renewcommand{\theenumi}{\roman{enumi}}
\renewcommand{\labelenumi}{\textnormal{(\theenumi)}$\;\;$}

\begin{eqnarray*}
\log\,L
	&=&
	\log\,P\!\left(\;
		\overset{n}{\underset{i=1}{\bigcap}}\;
		\left\{
			Y^{(i)}=c_{i},X^{(i)}=x_{i},\widetilde{Y}^{(i)}=y_{i},K^{(i)}=k_{i}
		\right\}
	\;\right)
\\
&=&
	{\color{white}+} \;\;
	\overset{C}{\underset{c=1}{\sum}}\;\;
	\overset{G}{\underset{g=1}{\sum}}\;\;
	\overset{C}{\underset{y=1}{\sum}}\;
	\left(\overset{n}{\underset{i=1}{\sum}}\;W^{(i)}_{c \vert gy{\color{red}0}}\right)
	\cdot
	\left(\,
		\log\left(\pi_{c \vert g}\,\mu_{0 \vert gy} + \delta_{cy}\,\mu_{1\vert gy}\right)
		\,\overset{{\color{white}.}}{+}\,
		\log\,\nu_{gy}
		\,\overset{{\color{white}.}}{+}\,
		\log\,\omega_{0}
	\,\right)
\\
&&
	+ \;\;
	\overset{C}{\underset{c=1}{\sum}}\;\;
	\overset{G}{\underset{g=1}{\sum}}\;\;
	\overset{C}{\underset{y=1}{\sum}}\;
	\left(\overset{n}{\underset{i=1}{\sum}}\;W^{(i)}_{c \vert gy{\color{red}1}}\right)
	\cdot
	\left(\,
		\log\,\pi_{c \vert g}
		\,\overset{{\color{white}.}}{+}\,
		\log\,\mu_{0\vert gy}
		\,\overset{{\color{white}.}}{+}\,
		\log\,\nu_{gy}
		\,\overset{{\color{white}.}}{+}\,
		\log\,\omega_{1}
	\,\right)
\\
&&
	+ \;\;
	\overset{C}{\underset{y=1}{\sum}}\;\;
	\overset{G}{\underset{g=1}{\sum}}\;
	\left(\overset{n}{\underset{i=1}{\sum}}\;W^{(i)}_{y \vert gy{\color{red}2}}\right)
	\cdot
	\left(\,
		\log\,\mu_{1 \vert gy}
		\,\overset{{\color{white}.}}{+}\,
		\log\,\nu_{gy}
		\,\overset{{\color{white}.}}{+}\,
		\log\,\omega_{1}
	\,\right)
\end{eqnarray*}

\begin{eqnarray*}
E\!\left[\,\left.\log\,L\;\right\vert\;\mathcal{D}\,\right]
&=& T_{1} \;+\; T_{2} \;+\; T_{3}
\\
T_{1}
&:=&
	\overset{C}{\underset{c=1}{\sum}}\;\;
	\overset{G}{\underset{g=1}{\sum}}\;\;
	\overset{C}{\underset{y=1}{\sum}}\;\;
	E_{c \vert gy{\color{red}0}}
	\cdot
	\left(\,
		\log\left(\pi_{c \vert g}\,\mu_{0 \vert gy} + \delta_{cy}\,\mu_{1\vert gy}\right)
		\,\overset{{\color{white}.}}{+}\,
		\log\,\nu_{gy}
		\,\overset{{\color{white}.}}{+}\,
		\log\,\omega_{0}
	\,\right)
\\
T_{2}
&:=&
	\overset{C}{\underset{c=1}{\sum}}\;\;
	\overset{G}{\underset{g=1}{\sum}}\;\;
	\overset{C}{\underset{y=1}{\sum}}\;\;
	E_{c \vert gy{\color{red}1}}
	\cdot
	\left(\,
		\log\,\pi_{c \vert g}
		\,\overset{{\color{white}.}}{+}\,
		\log\,\mu_{0\vert gy}
		\,\overset{{\color{white}.}}{+}\,
		\log\,\nu_{gy}
		\,\overset{{\color{white}.}}{+}\,
		\log\,\omega_{1}
	\,\right)
\\
T_{3}
&:=&
	\overset{C}{\underset{y=1}{\sum}}\;\;
	\overset{G}{\underset{g=1}{\sum}}\;\;
	E_{y \vert gy{\color{red}2}}
	\cdot
	\left(\,
		\log\,\mu_{1 \vert gy}
		\,\overset{{\color{white}.}}{+}\,
		\log\,\nu_{gy}
		\,\overset{{\color{white}.}}{+}\,
		\log\,\omega_{1}
	\,\right)
\end{eqnarray*}

\begin{eqnarray*}
T_{1}
&:=&
	\overset{C}{\underset{c=1}{\sum}}\;\;
	\overset{G}{\underset{g=1}{\sum}}\;\;
	\overset{C}{\underset{y=1}{\sum}}\;\;
	E_{c \vert gy{\color{red}0}}
	\cdot
	\left(\,
		\log\left(\pi_{c \vert g}\,\mu_{0 \vert gy} + \delta_{cy}\,\mu_{1\vert gy}\right)
		\,\overset{{\color{white}.}}{+}\,
		\log\,\nu_{gy}
		\,\overset{{\color{white}.}}{+}\,
		\log\,\omega_{0}
	\,\right)
\\
&=&
	\overset{C}{\underset{c=1}{\sum}}\;\;
	\overset{G}{\underset{g=1}{\sum}}\;\;
	\overset{C}{\underset{y=1}{\sum}}\;\;
	E_{c \vert gy{\color{red}0}}
	\cdot
	\left(\,
		\overset{{\color{white}.}}{\log}\left(\pi_{c \vert g}\,\mu_{0 \vert gy} + \delta_{cy}\,\mu_{1\vert gy}\right)
	\,\right)
	\;\; + \;\;
	\overset{C}{\underset{c=1}{\sum}}\;\;
	\overset{G}{\underset{g=1}{\sum}}\;\;
	\overset{C}{\underset{y=1}{\sum}}\;\;
	E_{c \vert gy{\color{red}0}}
	\cdot
	\left(\,
		\log\,\nu_{gy}
		\,\overset{{\color{white}.}}{+}\,
		\log\,\omega_{0}
	\,\right)	
\\
&=&
	\overset{G}{\underset{g=1}{\sum}}\;\;
	\overset{C}{\underset{y=1}{\sum}}\;\;
	\overset{C}{\underset{c=1}{\sum}}\;\;
	E_{c \vert gy{\color{red}0}}
	\cdot
	\left(\,
		\overset{{\color{white}.}}{\log}\left(\pi_{c \vert g}\,\mu_{0 \vert gy} + \delta_{cy}\,\mu_{1\vert gy}\right)
	\,\right)
	\;\; + \;\;
	\overset{C}{\underset{c=1}{\sum}}\;\;
	\overset{G}{\underset{g=1}{\sum}}\;\;
	\overset{C}{\underset{y=1}{\sum}}\;\;
	E_{c \vert gy{\color{red}0}}
	\cdot
	\left(\,
		\log\,\nu_{gy}
		\,\overset{{\color{white}.}}{+}\,
		\log\,\omega_{0}
	\,\right)	
\\
&=&
	{\color{white}+} \;\;
	\overset{G}{\underset{g=1}{\sum}}\;\;
	\overset{C}{\underset{y=1}{\sum}}\;
	\left\{
	E_{C \vert gy{\color{red}0}}
	\cdot
	\left(\,
		\overset{{\color{white}.}}{\log}\left(
			\left(1-\overset{C-1}{\underset{a=1}{\sum}}\pi_{a \vert g}\right)\,\mu_{0 \vert gy}
			+
			\delta_{Cy}\,\mu_{1\vert gy}
			\right)
	\,\right)
	\;+\;
	\overset{C-1}{\underset{a=1}{\sum}}\;\;
	E_{a \vert gy{\color{red}0}}
	\cdot
	\left(\,
		\overset{{\color{white}.}}{\log}\left(\pi_{a \vert g}\,\mu_{0 \vert gy}
		+
		\delta_{ay}\,\mu_{1\vert gy}\right)
	\,\right)
	\right\}
\\
&&
	+ \;\;
	\overset{C}{\underset{c=1}{\sum}}\;\;
	\overset{G}{\underset{g=1}{\sum}}\;\;
	\overset{C}{\underset{y=1}{\sum}}\;\;
	E_{c \vert gy{\color{red}0}}
	\cdot
	\left(\,
		\log\,\nu_{gy}
		\,\overset{{\color{white}.}}{+}\,
		\log\,\omega_{0}
	\,\right)	
\end{eqnarray*}

\begin{eqnarray*}
\dfrac{\partial\,T_{1}}{\partial\,\pi_{c \vert g}}
&=&
	\overset{C}{\underset{y=1}{\sum}}\;
	\left\{
	E_{C \vert gy{\color{red}0}}
	\cdot
	\left(\,
		\overset{{\color{white}.}}{\log}\left(
			\left(1-\overset{C-1}{\underset{a=1}{\sum}}\pi_{a \vert g}\right)\,\mu_{0 \vert gy}
			+
			\delta_{Cy}\,\mu_{1\vert gy}
			\right)
	\,\right)
	\;+\;
	\overset{C-1}{\underset{a=1}{\sum}}\;\;
	E_{a \vert gy{\color{red}0}}
	\cdot
	\left(\,
		\overset{{\color{white}.}}{\log}\left(\pi_{a \vert g}\,\mu_{0 \vert gy} + \delta_{ay}\,\mu_{1\vert gy}\right)
	\,\right)
	\right\}
\\
&=&
	\overset{C}{\underset{y=1}{\sum}}\;
	\left\{\;
	E_{C \vert gy{\color{red}0}}
	\cdot
	\dfrac{(-\,\mu_{0 \vert gy})}{
		\left(1-\overset{C-1}{\underset{a=1}{\sum}}\pi_{a \vert g}\right)\,\mu_{0 \vert gy}+\delta_{Cy}\,\mu_{1\vert gy}
		}
	\;+\;
	E_{c \vert gy{\color{red}0}}
	\cdot
	\dfrac{\mu_{0 \vert gy}}{\pi_{c \vert g}\,\mu_{0 \vert gy} + \delta_{cy}\,\mu_{1\vert gy}}
	\;\right\}
\\
&=&
	\overset{C}{\underset{y=1}{\sum}}\;\;
	\mu_{0 \vert gy}
	\cdot
	\left\{\;
		\dfrac{E_{c \vert gy{\color{red}0}}}{\pi_{c \vert g}\,\mu_{0 \vert gy} + \delta_{cy}\,\mu_{1\vert gy}}
		\;-\;
		\dfrac{E_{C \vert gy{\color{red}0}}}{
			\pi_{C \vert g}\,\mu_{0 \vert gy}+\delta_{Cy}\,\mu_{1\vert gy}
			%\left(1-\overset{C-1}{\underset{a=1}{\sum}}\pi_{a \vert g}\right)\,\mu_{0 \vert gy}+\delta_{Cy}\,\mu_{1\vert gy}
			}
	\;\right\}
\end{eqnarray*}

\begin{eqnarray*}
T_{2}
&:=&
	\overset{C}{\underset{a=1}{\sum}}\;\;
	\overset{G}{\underset{g=1}{\sum}}\;\;
	\overset{C}{\underset{y=1}{\sum}}\;\;
	E_{a \vert gy{\color{red}1}}
	\cdot
	\left(\,
		\log\,\pi_{a \vert g}
		\,\overset{{\color{white}.}}{+}\,
		\log\,\mu_{0\vert gy}
		\,\overset{{\color{white}.}}{+}\,
		\log\,\nu_{gy}
		\,\overset{{\color{white}.}}{+}\,
		\log\,\omega_{1}
	\,\right)
\\
&=&
	\overset{G}{\underset{g=1}{\sum}}\;\;
	\overset{C}{\underset{y=1}{\sum}}\;\;
	\overset{C}{\underset{a=1}{\sum}}\;\;
	E_{a \vert gy{\color{red}1}} \cdot \log\,\pi_{a \vert g}
	\; + \;
	\overset{G}{\underset{g=1}{\sum}}\;\;
	\overset{C}{\underset{y=1}{\sum}}\;\;
	\overset{C}{\underset{c=1}{\sum}}\;\;
	E_{a \vert gy{\color{red}1}}
	\cdot
	\left(\,
		\log\,\mu_{0\vert gy}
		\,\overset{{\color{white}.}}{+}\,
		\log\,\nu_{gy}
		\,\overset{{\color{white}.}}{+}\,
		\log\,\omega_{1}
	\,\right)
\\
&=&
	{\color{white}+} \;\;
	\overset{G}{\underset{g=1}{\sum}}\;\;
	\overset{C}{\underset{y=1}{\sum}}\;
	\left\{\;
		E_{C \vert gy{\color{red}1}} \cdot \log\left(1 - \overset{C-1}{\underset{a=1}{\sum}}\,\pi_{a \vert g}\right)
		\; + \;
		\overset{C-1}{\underset{a=1}{\sum}}\;
		E_{a \vert gy{\color{red}1}} \cdot \log\,\pi_{a \vert g}
	\;\right\}
\\
&&
	+ \;\;
	\overset{G}{\underset{g=1}{\sum}}\;\;
	\overset{C}{\underset{y=1}{\sum}}\;
	\left(\,\overset{C}{\underset{a=1}{\sum}}\; E_{a \vert gy{\color{red}1}}\,\right)
	\cdot
	\left(\,
		\log\,\mu_{0\vert gy}
		\,\overset{{\color{white}.}}{+}\,
		\log\,\nu_{gy}
		\,\overset{{\color{white}.}}{+}\,
		\log\,\omega_{1}
	\,\right)
\end{eqnarray*}

\begin{eqnarray*}
\dfrac{\partial\,T_{2}}{\partial\,\pi_{c \vert g}}
&=&
	\overset{C}{\underset{y=1}{\sum}}\;
	\left\{\;
		\dfrac{-\,E_{C \vert gy{\color{red}1}}}{1 - \overset{C-1}{\underset{a=1}{\sum}}\,\pi_{a \vert g}}
		\; + \;
		\dfrac{E_{c \vert gy{\color{red}1}}}{\pi_{c \vert g}}
	\,\right\}
	\;\; = \;\;
	\overset{C}{\underset{y=1}{\sum}}\;
	\left\{\;
		\dfrac{E_{c \vert gy{\color{red}1}}}{\pi_{c \vert g}}
		\; - \;
		\dfrac{\,E_{C \vert gy{\color{red}1}}}{\pi_{C \vert g}}
	\,\right\}
\\
&=&
	\dfrac{1}{\pi_{c \vert g}}
	\cdot
	\left\{\;
		\overset{C}{\underset{y=1}{\sum}}\;
		E_{c \vert gy{\color{red}1}}
	\,\right\}
	\;\; - \;\;
	\dfrac{1}{\pi_{C \vert g}}
	\cdot
	\left\{\;
		\overset{C}{\underset{y=1}{\sum}}\;
		E_{C \vert gy{\color{red}1}}
	\,\right\}
\end{eqnarray*}

\begin{eqnarray*}
\dfrac{\partial\;E\!\left[\,\left.\log\,L\;\right\vert\;\mathcal{D}\,\right]}{\partial\;\pi_{c \vert g}}
&=& \dfrac{\partial\;T_{1}}{\partial\;\pi_{c \vert g}} \;+\; \dfrac{\partial\;T_{2}}{\partial\;\pi_{c \vert g}}
\\
&=&
	{\color{white}+} \;\;
	\overset{C}{\underset{y=1}{\sum}}\;\;
	\mu_{0 \vert gy}
	\cdot
	\left\{\;
		\dfrac{E_{c \vert gy{\color{red}0}}}{\pi_{c \vert g}\,\mu_{0 \vert gy} + \delta_{cy}\,\mu_{1\vert gy}}
		\;-\;
		\dfrac{E_{C \vert gy{\color{red}0}}}{
			\pi_{C \vert g}\,\mu_{0 \vert gy}+\delta_{Cy}\,\mu_{1\vert gy}
			}
	\;\right\}
\\
&&
	+ \;\;
	\dfrac{1}{\pi_{c \vert g}}
	\cdot
	\left\{\;
		\overset{C}{\underset{y=1}{\sum}}\;
		E_{c \vert gy{\color{red}1}}
	\,\right\}
	\;\; - \;\;
	\dfrac{1}{\pi_{C \vert g}}
	\cdot
	\left\{\;
		\overset{C}{\underset{y=1}{\sum}}\;
		E_{C \vert gy{\color{red}1}}
	\,\right\}
\\
&=&
	{\color{white}-} \;\;
	\left\{\;\,
		\overset{C}{\underset{y=1}{\sum}}\;
		\dfrac{\mu_{0 \vert gy} \cdot E_{c \vert gy{\color{red}0}}}{
			{\color{white}.}
			\pi_{c \vert g}\,\mu_{0 \vert gy} + \delta_{cy}\,\mu_{1\vert gy}
			{\color{white}.}
			}
		\; + \;
		\dfrac{1}{
			{\color{white}\vert}\!
			\pi_{c \vert g}
			\!{\color{white}\vert}
			}
		\cdot
			\overset{C}{\underset{y=1}{\sum}}\;
			\,E_{c \vert gy{\color{red}1}}\,
	\right\}
\\
&&
	- \;\;
	\left\{\;\,
		\overset{C}{\underset{y=1}{\sum}}\;
		\dfrac{\mu_{0 \vert gy} \cdot E_{C \vert gy{\color{red}0}}}
			{\pi_{C \vert g}\,\mu_{0 \vert gy} + \delta_{Cy}\,\mu_{1\vert gy}}
		\; + \;
		\dfrac{1}{\pi_{C \vert g}}
		\cdot
			\overset{C}{\underset{y=1}{\sum}}\;
			E_{C \vert gy{\color{red}1}}
	\right\}
\end{eqnarray*}

\begin{eqnarray*}
&&
	\dfrac{\partial\;E\!\left[\,\left.\log\,L\;\right\vert\;\mathcal{D}\,\right]}{\partial\;\pi_{c \vert g}} \;=\; 0\,,
	\quad\forall\;\,c\;\in\,\{1,\ldots,C-1\}
\\
&\Longrightarrow&
	\;{\color{white}=} \;\;
		\overset{C}{\underset{y=1}{\sum}}\;\;
		\dfrac{\mu_{0 \vert gy} \cdot E_{c \vert gy{\color{red}0}}}{
			{\color{white}.}
			\pi_{c \vert g}\,\mu_{0 \vert gy} + \delta_{cy}\,\mu_{1\vert gy}
			{\color{white}.}
			}
		\; + \;
		\dfrac{1}{
			{\color{white}\vert}\!
			\pi_{c \vert g}
			\!{\color{white}\vert}
			}
		\cdot
			\overset{C}{\underset{y=1}{\sum}}\;
			\,E_{c \vert gy{\color{red}1}}\,
\\
&&
	= \;\;
		\overset{C}{\underset{y=1}{\sum}}\;\;
		\dfrac{\mu_{0 \vert gy} \cdot E_{C \vert gy{\color{red}0}}}{\pi_{C \vert g}\,\mu_{0 \vert gy} + \delta_{Cy}\,\mu_{1\vert gy}}
		\; + \;
		\dfrac{1}{\pi_{C \vert g}}
		\cdot
			\overset{C}{\underset{y=1}{\sum}}\;
			E_{C \vert gy{\color{red}1}}\,,
		\quad\forall\;\,c\;\in\,\{1,\ldots,C-1\}
\\
&\Longrightarrow&
		\overset{C}{\underset{y=1}{\sum}}\;\;
		\dfrac{\mu_{0 \vert gy} \cdot E_{c \vert gy{\color{red}0}}}{
			\pi_{c \vert g}\,\mu_{0 \vert gy} + \delta_{cy}\,\mu_{1\vert gy}
			}
		\; + \;
		\dfrac{1}{\pi_{c \vert g}}
		\cdot
			\overset{C}{\underset{y=1}{\sum}}\;
			\,E_{c \vert gy{\color{red}1}}\,
		\;\; = \;\;
		A_{g}\,,
		\quad\forall\;\,c\;\in\,\{1,\ldots,C\}
\\
&\Longrightarrow&
		\dfrac{\mu_{0 \vert gc} \cdot E_{c \vert gc{\color{red}0}}}{
			\pi_{c \vert g}\,\mu_{0 \vert gc} + 1\cdot\mu_{1\vert gc}
			}
		\; + \;
		\overset{C}{\underset{y=1,y\neq c}{\sum}}\;
		\dfrac{\mu_{0 \vert gy} \cdot E_{c \vert gy{\color{red}0}}}{
			\pi_{c \vert g}\,\mu_{0 \vert gy} + 0\cdot\mu_{1\vert gy}
			}
		\; + \;
		\dfrac{1}{\pi_{c \vert g}}
		\cdot
			\overset{C}{\underset{y=1}{\sum}}\;
			\,E_{c \vert gy{\color{red}1}}\,
		\;\; = \;\;
		A_{g}\,,
		\quad\forall\;\,c\;\in\,\{1,\ldots,C\}
\\
&\Longrightarrow&
		\dfrac{\mu_{0 \vert gc} \cdot E_{c \vert gc{\color{red}0}}}{
			\pi_{c \vert g}\,\mu_{0 \vert gc} + \mu_{1\vert gc}
			}
		\; + \;
		\overset{C}{\underset{y=1,y\neq c}{\sum}}\;
		\dfrac{E_{c \vert gy{\color{red}0}}}{\pi_{c \vert g}}
		\; + \;
		\dfrac{1}{\pi_{c \vert g}}
		\cdot
			\overset{C}{\underset{y=1}{\sum}}\;
			\,E_{c \vert gy{\color{red}1}}\,
		\;\; = \;\;
		A_{g}\,,
		\quad\forall\;\,c\;\in\,\{1,\ldots,C\}
\\
&\Longrightarrow&
		\dfrac{\mu_{0 \vert gc} \cdot E_{c \vert gc{\color{red}0}}}{
			\pi_{c \vert g}\,\mu_{0 \vert gc} + \mu_{1\vert gc}
			}
		\; - \;
		\dfrac{E_{c \vert gc{\color{red}0}}}{\pi_{c \vert g}}
		\; + \;
		\overset{C}{\underset{y=1}{\sum}}\;
		\dfrac{E_{c \vert gy{\color{red}0}}}{\pi_{c \vert g}}
		\; + \;
		\dfrac{1}{\pi_{c \vert g}}
		\cdot
			\overset{C}{\underset{y=1}{\sum}}\;
			\,E_{c \vert gy{\color{red}1}}\,
		\;\; = \;\;
		A_{g}\,,
		\quad\forall\;\,c\;\in\,\{1,\ldots,C\}
\\
&\Longrightarrow&
		\left(\;
			\dfrac{\mu_{0 \vert gc} \cdot E_{c \vert gc{\color{red}0}}}{
				\pi_{c \vert g}\,\mu_{0 \vert gc} + \mu_{1\vert gc}
				}
			\; - \;
			\dfrac{E_{c \vert gc{\color{red}0}}}{\pi_{c \vert g}}
		\;\right)
		\; + \;
		\dfrac{1}{\pi_{c \vert g}}
		\left(\;
			\overset{C}{\underset{y=1}{\sum}}\;\;
			\overset{1}{\underset{k=0}{\sum}}\;
			E_{c \vert gyk}
		\,\right)
		\;\; = \;\;
		A_{g}\,,
		\quad\forall\;\,c\;\in\,\{1,\ldots,C\}
\\
&\Longrightarrow&
		\left(\;
			\dfrac{\mu_{0 \vert gc} \cdot E_{c \vert gc{\color{red}0}}}{
				\pi_{c \vert g}\,\mu_{0 \vert gc} + \mu_{1\vert gc}
				}
		\;\right)
		\; + \;
		\dfrac{1}{\pi_{c \vert g}}
		\left(\;
			-\,E_{c \vert gc{\color{red}0}}
			\; + \;
			\overset{C}{\underset{y=1}{\sum}}\;\;
			\overset{1}{\underset{k=0}{\sum}}\;
			E_{c \vert gyk}
		\,\right)
		\;\; = \;\;
		A_{g}\,,
		\quad\forall\;\,c\;\in\,\{1,\ldots,C\}
\end{eqnarray*}

          %%%%% ~~~~~~~~~~~~~~~~~~~~ %%%%%
