
          %%%%% ~~~~~~~~~~~~~~~~~~~~ %%%%%

\section{Technical Lemmas}
\setcounter{theorem}{0}
\setcounter{equation}{0}

\renewcommand{\theenumi}{\roman{enumi}}
\renewcommand{\labelenumi}{\textnormal{(\theenumi)}$\;\;$}

\begin{lemma}\label{LemmaPhi}
Define
\begin{equation*}
\phi \, : \; [\,0,\infty\,) \, \longrightarrow \, [\,0,1\,] \, : \, t \, \longmapsto \,\min\{\,1\,,t\,\}. 
\end{equation*}
Then, $\phi$ satisfies:
\begin{equation*}
\phi(s + t) \; \leq \; \phi(s) \,+\, \phi(t),
\;\;\textnormal{for each $s, t \in [0,\infty)$}.
\end{equation*}
\end{lemma}
\proof
For any $s, t \in [0,\infty)$, either $s + t \geq 1$ or $s + t <1$. 
If $s + t \geq 1$, then
\begin{equation*}
\phi(s+t)
\;=\; \min\{1,s + t\}
\;=\; 1
\;<\; 2
\;=\; 1 + 1
\;\leq\; \min\{1,s\} + \min\{1,t\}
\;=\; \phi(s) + \phi(t),
\end{equation*}
hence, the required inequality holds.
On the other hand, if $s + t < 1$, then we must also have $s < 1$ and $t < 1$ (since $s, t \geq 0$).
Hence,
\begin{equation*}
\phi(s+t)
\;=\; \min\{1,s + t\}
\;=\; s+t
\;=\; \min\{1,s\} + \min\{1,t\}
\;=\; \phi(s) + \phi(t),
\end{equation*}
thus, the required inequality also holds.
\qed

\begin{lemma}\label{LemmaMin}
For any $x, y, z \in \Re$, we have:
\begin{equation*}
\min\{1,\vert\,x-y\,\vert\}
\;\leq\;
\min\{1,\vert\,x-z\,\vert\}
\;+\;
\min\{1,\vert\,z-y\,\vert\}.
\end{equation*}
\end{lemma}
\proof
Observe that $\vert\,x - y\,\vert \;\leq\; \vert\,x-z\,\vert+\vert\,z-y\,\vert$ implies
\begin{equation*}
\min\{\,1\,,\vert\,x - y\,\vert\,\} \;\leq\; \vert\,x-z\,\vert+\vert\,z-y\,\vert.
\end{equation*}
The above inequality, together with $\min\{\,1\,,\vert\,x - y\,\vert\,\} \;\leq\; 1$,
thus in turn imply:
\begin{equation*}
\min\{\,1\,,\vert\,x - y\,\vert\,\} \;\leq\; \min\{\,1\,,\vert\,x-z\,\vert+\vert\,z-y\,\vert\,\}.
\end{equation*}
By Lemma \ref{LemmaPhi}, we therefore have:
\begin{equation*}
\min\{\,1\,,\vert\,x - y\,\vert\,\}
\;\leq\; \min\{\,1\,,\vert\,x-z\,\vert+\vert\,z-y\,\vert\,\}.
\;\leq\; \min\{\,1\,,\vert\,x-z\,\vert\,\} \;+\; \min\{\,1\,,\vert\,z-y\,\vert\,\},
\end{equation*}
which proves the present Lemma.
\qed

          %%%%% ~~~~~~~~~~~~~~~~~~~~ %%%%%
