
          %%%%% ~~~~~~~~~~~~~~~~~~~~ %%%%%

\section{Technical Lemmas}
\setcounter{theorem}{0}
\setcounter{equation}{0}

\renewcommand{\theenumi}{\roman{enumi}}
\renewcommand{\labelenumi}{\textnormal{(\theenumi)}$\;\;$}

\begin{lemma}\label{LemmaPhi}
Define
\begin{equation*}
\phi \, : \; [\,0,\infty\,) \, \longrightarrow \, [\,0,1\,] \, : \, t \, \longmapsto \,\min\{\,1\,,t\,\}. 
\end{equation*}
Then, $\phi$ satisfies:
\begin{equation*}
\phi(s + t) \; \leq \; \phi(s) \,+\, \phi(t),
\;\;\textnormal{for each $s, t \in [0,\infty)$}.
\end{equation*}
\end{lemma}
\proof
For any $s, t \in [0,\infty)$, either $s + t \geq 1$ or $s + t <1$. 
If $s + t \geq 1$, then
\begin{equation*}
\phi(s+t)
\;=\; \min\{1,s + t\}
\;=\; 1
\;<\; 2
\;=\; 1 + 1
\;\leq\; \min\{1,s\} + \min\{1,t\}
\;=\; \phi(s) + \phi(t),
\end{equation*}
hence, the required inequality holds.
On the other hand, if $s + t < 1$, then we must also have $s < 1$ and $t < 1$ (since $s, t \geq 0$).
Hence,
\begin{equation*}
\phi(s+t)
\;=\; \min\{1,s + t\}
\;=\; s+t
\;=\; \min\{1,s\} + \min\{1,t\}
\;=\; \phi(s) + \phi(t),
\end{equation*}
thus, the required inequality also holds.
\qed

\begin{lemma}\label{LemmaMin}
For any $x, y, z \in \Re$, we have:
\begin{equation*}
\min\{1,\vert\,x-y\,\vert\}
\;\leq\;
\min\{1,\vert\,x-z\,\vert\}
\;+\;
\min\{1,\vert\,z-y\,\vert\}.
\end{equation*}
\end{lemma}
\proof
Observe that $\vert\,x - y\,\vert \;\leq\; \vert\,x-z\,\vert+\vert\,z-y\,\vert$ implies
\begin{equation*}
\min\{\,1\,,\vert\,x - y\,\vert\,\} \;\leq\; \vert\,x-z\,\vert+\vert\,z-y\,\vert.
\end{equation*}
The above inequality, together with $\min\{\,1\,,\vert\,x - y\,\vert\,\} \;\leq\; 1$,
thus in turn imply:
\begin{equation*}
\min\{\,1\,,\vert\,x - y\,\vert\,\} \;\leq\; \min\{\,1\,,\vert\,x-z\,\vert+\vert\,z-y\,\vert\,\}.
\end{equation*}
By Lemma \ref{LemmaPhi}, we therefore have:
\begin{equation*}
\min\{\,1\,,\vert\,x - y\,\vert\,\}
\;\leq\; \min\{\,1\,,\vert\,x-z\,\vert+\vert\,z-y\,\vert\,\}.
\;\leq\; \min\{\,1\,,\vert\,x-z\,\vert\,\} \;+\; \min\{\,1\,,\vert\,z-y\,\vert\,\},
\end{equation*}
which proves the present Lemma.
\qed

\begin{lemma}[The Weierstrass $M$-test, Theorem A.28, \cite{Billingsley2012}]\label{WeierstrassMTest}
\mbox{}\vskip 0.1cm
\noindent
Suppose that $\underset{n\rightarrow\infty}{\lim}\,x^{(n)}_{i} \,=\, x_{i}$,\; for each $i \in \N$,
and that $\left\vert\,x^{(n)}_{i}\,\right\vert \,\leq\, M_{i}$,
where $\overset{\infty}{\underset{i=1}{\sum}}\,M_{i} < \infty$.
Then,
\begin{enumerate}
\item
	$\overset{\infty}{\underset{i=1}{\sum}}\, x_{i}$ exists, \;and\;\;
	$\overset{\infty}{\underset{i=1}{\sum}}\, x^{(n)}_{i}$ exists for each $n \in \N$.
\item	Furthermore,
	\begin{equation*}
	\underset{n\rightarrow\infty}{\lim}\;\overset{\infty}{\underset{i=1}{\sum}}\, x^{(n)}_{i}
	\; = \;\;
	\overset{\infty}{\underset{i=1}{\sum}}\, x_{i}.
	\end{equation*}
\end{enumerate}
\end{lemma}
\proof
\begin{enumerate}
\item
	$\overset{\infty}{\underset{i=1}{\sum}}\,M_{i} < \infty$ \;\;and\;\; $\left\vert\,x^{(n)}_{i}\,\right\vert \leq M_{i}$
	\quad$\Longrightarrow$\quad the series \;$\overset{\infty}{\underset{i=1}{\sum}}\, x_{i}$ \;and\;
	$\overset{\infty}{\underset{i=1}{\sum}}\, x^{(n)}_{i}$, $n \in \N$, \;converge absolutely.
\item
	Let $\varepsilon > 0$ be given. Choose $K \in \N$ sufficiently large such that
	$\overset{\infty}{\underset{j = K + 1}{\sum}}\,M_{i} < \dfrac{\varepsilon}{3}$.
	Next, choose $N \in \N$ sufficiently large such that
	\begin{equation*}
	\left\vert\;x^{(n)}_{i} \,-\, x_{i}\;\right\vert
	\; < \; \dfrac{\varepsilon}{3K},
	\;\;\textnormal{for any $n > N$ and $i = 1, 2, \ldots, K$}.
	\end{equation*}
	Then, we have, for each $n > N$,
	\begin{eqnarray*}
	\left\vert\;\;
	\sum^{\infty}_{i=1}\,x^{(n)}_{i} \, - \, \sum^{\infty}_{i=1}x_{i}
	\;\right\vert
	&=&
	\left\vert\;\;
	\sum^{K}_{i=1}\left(\,x^{(n)}_{i} \, - \, x_{i}\,\right) \, + \, \sum_{i=K+1}^{\infty}x^{(n)}_{i} \, - \, \sum^{\infty}_{i=K+1}x_{i}
	\;\right\vert
	\\
	&\leq&
	\sum^{K}_{i=1}
	\left\vert\; x^{(n)}_{i} \, - \, x_{i}\;\right\vert
	\;+\; \sum^{\infty}_{i=K+1}\left\vert\, x^{(n)}_{i} \,\right\vert
	\;+\; \sum^{\infty}_{i=K+1}\left\vert\, x_{i} \,\right\vert
	\\
	&\leq&
	K \cdot \dfrac{\varepsilon}{3K}
	\;+\; \sum^{\infty}_{i=K+1}M_{i}
	\;+\; \sum^{\infty}_{i=K+1}M_{i}
	\;\;\leq\;\;
	\dfrac{\varepsilon}{3} + 2\cdot\dfrac{\varepsilon}{3}
	\;\;=\;\; \varepsilon.
	\end{eqnarray*}
	Since $\varepsilon$ is arbitrary, this proves:
	\begin{equation*}
	\underset{n\rightarrow\infty}{\lim}\;\overset{\infty}{\underset{i=1}{\sum}}\, x^{(n)}_{i}
	\; = \;\;
	\overset{\infty}{\underset{i=1}{\sum}}\, x_{i}.
	\end{equation*}
\end{enumerate}
\qed

          %%%%% ~~~~~~~~~~~~~~~~~~~~ %%%%%
