
          %%%%% ~~~~~~~~~~~~~~~~~~~~ %%%%%

\section{Exercises}
\setcounter{theorem}{0}
\setcounter{equation}{0}

%\cite{vanDerVaart1996}
%\cite{Kosorok2008}

%\renewcommand{\theenumi}{\alph{enumi}}
%\renewcommand{\labelenumi}{\textnormal{(\theenumi)}$\;\;$}
\renewcommand{\theenumi}{\roman{enumi}}
\renewcommand{\labelenumi}{\textnormal{(\theenumi)}$\;\;$}

          %%%%% ~~~~~~~~~~~~~~~~~~~~ %%%%%

\noindent
\underline{{\color{white}.}\textbf{Exercise 6.7, p.144, \cite{Brzezniak1999}}{\color{white}.}}
\vskip 0.3cm
\noindent
Suppose \,$\left\{\,\overset{{\color{white}.}}{N}_{t}\,\right\}_{t\in[\,0,\infty)}$\, is a Poisson process
with intensity \,$\lambda > 0$.
\vskip 0.2cm
\noindent
For \,$s < t$,\, compute \,$P\!\left(\,N_{s} \overset{{\color{white}-}}{=} 1\,,\,N_{t} = 2\,\right)$\, in terms of \,$s,\,t$\, and \,$\lambda$.

\vskip 0.5cm
\noindent
\textit{Solution}\quad
First, note that
\begin{equation*}
\left\{\, N_{s} \overset{{\color{white}-}}{=} 1 \,,\, N_{t} = 2 \,\right\}
\;\; = \;\;
	\left\{\; \eta_{1} \,\leq\, s \,\overset{{\color{white}.}}{<}\, \eta_{1} + \eta_{2} \,\leq\, t \,<\, \eta_{1} + \eta_{2} + \eta_{3} \;\right\}
\end{equation*}
Hence,
\begin{eqnarray*}
&&
	P\!\left(\, N_{s} \overset{{\color{white}-}}{=} 1 \,,\, N_{t} = 2 \,\right)
\;\; = \;\;
	P\!\left(\; \eta_{1} \,\leq\, s \,\overset{{\color{white}.}}{<}\, \eta_{1} + \eta_{2} \,\leq\, t \,<\, \eta_{1} + \eta_{2} + \eta_{3} \;\right)
\\
& = &
	\int_{0}^{s}\; \int_{s-u_{1}}^{t-u_{1}} \int_{t-u_{1}-u_{2}}^{\infty}\;
	f_{\eta_{1},\eta_{2},\eta_{3}}(u_{1},u_{2},u_{3})
	\;\d\,u_{3}\;\d\,u_{2}\;\d\,u_{1}
\\
& = &
	\int_{0}^{s}\; \int_{s-u_{1}}^{t-u_{1}} \int_{t-u_{1}-u_{2}}^{\infty}\;
	f_{\eta_{1}}(u_{1}) \cdot f_{\eta_{2}}(u_{2}) \cdot f_{\eta_{3}}(u_{3})
	\;\d\,u_{3}\;\d\,u_{2}\;\d\,u_{1}\,,
	\quad
	\textnormal{by independence of \,$\eta_{1},\,\eta_{2},\,\eta_{3}$}
\\
& = &
	\int_{0}^{s}\; \int_{s-u_{1}}^{t-u_{1}}
		f_{\eta_{1}}(u_{1}) \cdot f_{\eta_{2}}(u_{2})
		\cdot
		\left(\;\int_{t-u_{1}-u_{2}}^{\infty}\; f_{\eta_{3}}(u_{3}) \;\d\,u_{3}\right)
		\;\d\,u_{2}\;\d\,u_{1}
\\
& = &
	\int_{0}^{s}\; \int_{s-u_{1}}^{t-u_{1}}
		f_{\eta_{1}}(u_{1}) \cdot f_{\eta_{2}}(u_{2})
		\cdot
		P\!\left(\,t\overset{{\color{white}.}}{-}u_{1}-u_{2}<\eta_{3}\,\right)
		\;\d\,u_{2}\;\d\,u_{1}
\\
& = &
	\int_{0}^{s}\; \int_{s-u_{1}}^{t-u_{1}}
		f_{\eta_{1}}(u_{1}) \cdot f_{\eta_{2}}(u_{2})
		\cdot
		\exp\!\left(\overset{{\color{white}.}}{-}\lambda(t-u_{1}-u_{2})\right)
		\;\d\,u_{2}\;\d\,u_{1}
\\
& = &
	\int_{0}^{s}\;
		f_{\eta_{1}}(u_{1}) \cdot 
		\left(\;\int_{s-u_{1}}^{t-u_{1}}
			f_{\eta_{2}}(u_{2})
			\cdot
			\exp\!\left(\overset{{\color{white}.}}{-}\lambda(t-u_{1}-u_{2})\right)
			\d\,u_{2}\right)
		\,\d\,u_{1}
\\
& = &
	\int_{0}^{s}\;
		f_{\eta_{1}}(u_{1}) \cdot \exp\!\left(\overset{{\color{white}.}}{-}\lambda(t-u_{1})\right)
		\left(\;\int_{s-u_{1}}^{t-u_{1}}
			\lambda\cdot\exp\!\left(\overset{{\color{white}.}}{-}\lambda u_{2}\right)
			\cdot
			\exp\!\left(\overset{{\color{white}.}}{+}\lambda u_{2}\right)
			\d\,u_{2}\right)
		\,\d\,u_{1}
\\
& = &
	\int_{0}^{s}\;
		f_{\eta_{1}}(u_{1}) \cdot \exp\!\left(\overset{{\color{white}.}}{-}\lambda(t-u_{1})\right)
		\cdot
		\lambda\cdot\left[\,(t-u_{1})\overset{{\color{white}.}}{-}(s-u_{1})\,\right]
		\,\d\,u_{1}
\\
& = &
	\lambda \cdot (t-s) \cdot \exp\!\left(\overset{{\color{white}.}}{-}\lambda t\right)
	\cdot
	\int_{0}^{s}\;
		\lambda \cdot \exp\!\left(\overset{{\color{white}.}}{-}\lambda u_{1}\right)
		\cdot
		\exp\!\left(\overset{{\color{white}.}}{+}\lambda u_{1}\right)
		\cdot
		\,\d\,u_{1}
\\
& \overset{{\color{white}1}}{=} &
	\lambda \cdot (t-s) \cdot \exp\!\left(\overset{{\color{white}.}}{-}\lambda t\right)
	\cdot
	\lambda \cdot s
\\
& \overset{{\color{white}1}}{=} &
	\lambda^{2} \cdot s \cdot (t-s) \cdot \exp\!\left(\overset{{\color{white}.}}{-}\lambda t\right)
\end{eqnarray*}
\qed

          %%%%% ~~~~~~~~~~~~~~~~~~~~ %%%%%

%\renewcommand{\theenumi}{\alph{enumi}}
%\renewcommand{\labelenumi}{\textnormal{(\theenumi)}$\;\;$}
\renewcommand{\theenumi}{\roman{enumi}}
\renewcommand{\labelenumi}{\textnormal{(\theenumi)}$\;\;$}

          %%%%% ~~~~~~~~~~~~~~~~~~~~ %%%%%
