
\noindent
\textbf{Exercise 3.12}

\vskip 0.3cm
\noindent

Recall that
\begin{equation*}
\textnormal{Corr}\left(\overline{Y}_{a},\overline{Y}_{g}\right)
\;\;=\;\;
\dfrac{\textnormal{Cov}\left(\overline{Y}_{a},\overline{Y}_{g}\right)}
{\sqrt{V\!\left[\,\overline{Y}_{a}\,\right]\cdot V\!\left[\,\overline{Y}_{g}\,\right]}}
\end{equation*}
We first compute $V\!\left[\,\overline{Y}_{a}\,\right]$, followed by
$V\!\left[\,\overline{Y}_{g}\,\right]$, and then
$\textnormal{Cov}\left(\overline{Y}_{a},\overline{Y}_{g}\right)$.
Now, if $X \sim N(\mu,\sigma^{2})$ and $Y = \exp(X)$, then
\begin{equation*}
Y \sim \textnormal{LogNormal}(\mu,\sigma^{2})
\end{equation*}
and we then have
\begin{equation*}
E[\,Y\,] \;\; = \;\; e^{\mu + \frac{\sigma^{2}}{2}}
\quad\textnormal{and}\quad
V[\,Y\,]
\;\; = \;\; E[\,Y\,]^{2}\cdot\left(e^{\sigma^{2}}-1\right)
\;\; = \;\; \left(e^{\mu+\frac{\sigma^{2}}{2}}\right)^{2}\cdot\left(e^{\sigma^{2}}-1\right)
\;\; = \;\; \left(e^{2\mu+\sigma^{2}}\right)\cdot\left(e^{\sigma^{2}}-1\right)
\end{equation*}
Hence,
\begin{equation*}
V\left[\,\overline{Y}_{a}\,\right]
\;\; = \;\;
V\left[\,\dfrac{1}{n}\sum_{i=1}^{n}Y_{i}\,\right]
\;\; = \;\;
\dfrac{1}{n^{2}}\sum_{i=1}^{n}V\left[\,Y_{i}\,\right]
\;\; = \;\;
\dfrac{1}{n}V\left[\,Y\,\right]
\;\; = \;\;
\dfrac{1}{n} \left(e^{2\mu+\sigma^{2}}\right)\cdot\left(e^{\sigma^{2}}-1\right)
\end{equation*}
Next, note that, since $\overline{Y}_{g} = \left(\,\prod_{i=1}^{n}Y_{i}\,\right)^{1/n}$,
we have
\begin{equation*}
\log\left(\,\overline{Y}_{g}\,\right)
\;\; = \;\;
\log\left[\left(\prod_{i=1}^{n}Y_{i}\right)^{1/n}\right]
\;\; = \;\;
\dfrac{1}{n}\sum_{i=1}^{n}\log\left(\,Y_{i}\,\right)
\;\; = \;\;
\dfrac{1}{n}\sum_{i=1}^{n}X_{i}
\;\; = \;\;
\overline{X}_{n}
\;\; \sim \;\;
N\!\left(\,\mu\,,\,\dfrac{\sigma^{2}}{n}\,\right)
\end{equation*}
Thus,
\begin{equation*}
\overline{Y}_{g}
\;\; = \;\;
e^{\overline{X}_{n}}
\;\; = \;\;
\textnormal{LogNormal}\!\left(\,\mu\,,\,\dfrac{\sigma^{2}}{n}\,\right)
\end{equation*}
Hence,
\begin{equation*}
V\!\left[\,\overline{Y}_{g}\,\right]
\;\; = \;\;
\left[\,e^{\mu+\frac{\sigma^{2}}{2n}}\,\right]^{2}
\cdot
\left(e^{\frac{\sigma^{2}}{n}} - 1\right)
\;\; = \;\;
\left[\,e^{2\mu+\frac{\sigma^{2}}{n}}\,\right]
\cdot
\left(e^{\frac{\sigma^{2}}{n}} - 1\right)
\end{equation*}
Next,
\begin{equation*}
\textnormal{Cov}\left(\,\overline{Y_{a}}\,,\,\overline{Y}_{g}\,\right)
\;\;=\;\;
\textnormal{Cov}\left(\,
\dfrac{1}{n}\sum_{i=1}^{n}Y_{i}
\,,\,
\overline{Y}_{g}
\,\right)
\;\;=\;\;
\dfrac{1}{n}\sum_{i=1}^{n}
\textnormal{Cov}\left(\,
Y_{i}
\,,\,
\overline{Y}_{g} %\left(\,\prod_{k=1}^{n}Y_{k}\right)^{1/n}
\,\right)
\;\;=\;\;
\dfrac{1}{n}\sum_{i=1}^{n}
\left\{\,
E\!\left[\,Y_{i}\cdot \overline{Y}_{g}\,\right]
\;-\;
E\!\left[\,Y_{i}\,\right]\cdot E\!\left[\overline{Y}_{g}\,\right]
\,\right\}
\end{equation*}

%%%%%%%%%%%%%%%%%%%%%%%%%%%%%%%%%%%%%%%%%%%%%%%%%%%%%%%%%%%%%%%%%%%%%%%%%%%%%%%%%%%%%%%%%%%%%%%%%%%%

