
\noindent
\textbf{Exercise 3.12}

\vskip 0.3cm
\noindent

Recall that
\begin{equation*}
\textnormal{Corr}\left(\,\overline{Y}_{a},\overline{Y}_{g}\,\right)
\;\;=\;\;
\dfrac{\textnormal{Cov}\left(\,\overline{Y}_{a},\overline{Y}_{g}\,\right)}
{\sqrt{V\!\left[\,\overline{Y}_{a}\,\right]\cdot V\!\left[\,\overline{Y}_{g}\,\right]}}
\end{equation*}
We first compute $V\!\left[\,\overline{Y}_{a}\,\right]$, followed by
$V\!\left[\,\overline{Y}_{g}\,\right]$, and then
$\textnormal{Cov}\left(\overline{Y}_{a},\overline{Y}_{g}\right)$.
Now, if $X \sim N(\mu,\sigma^{2})$ and $Y = \exp(X)$, then
\begin{equation*}
Y \sim \textnormal{LogNormal}(\mu,\sigma^{2})
\end{equation*}
and we then have
\begin{equation*}
E[\,Y\,] \;\; = \;\; e^{\mu + \frac{\sigma^{2}}{2}}
\quad\textnormal{and}\quad
V[\,Y\,]
\;\; = \;\; E[\,Y\,]^{2}\cdot\left(e^{\sigma^{2}}-1\right)
\;\; = \;\; \left(e^{\mu+\frac{\sigma^{2}}{2}}\right)^{2}\cdot\left(e^{\sigma^{2}}-1\right)
\;\; = \;\; \left(e^{2\mu+\sigma^{2}}\right)\cdot\left(e^{\sigma^{2}}-1\right)
\end{equation*}
Hence,
\begin{equation*}
V\left[\,\overline{Y}_{a}\,\right]
\;\; = \;\;
V\left[\,\dfrac{1}{n}\sum_{i=1}^{n}Y_{i}\,\right]
\;\; = \;\;
\dfrac{1}{n^{2}}\sum_{i=1}^{n}V\left[\,Y_{i}\,\right]
\;\; = \;\;
\dfrac{1}{n}V\left[\,Y\,\right]
\;\; = \;\;
\dfrac{1}{n} \left(e^{2\mu+\sigma^{2}}\right)\cdot\left(e^{\sigma^{2}}-1\right)
\end{equation*}
Next, note that, since $\overline{Y}_{g} = \left(\,\prod_{i=1}^{n}Y_{i}\,\right)^{1/n}$,
we have
\begin{equation*}
\log\left(\,\overline{Y}_{g}\,\right)
\;\; = \;\;
\log\left[\left(\prod_{i=1}^{n}Y_{i}\right)^{1/n}\right]
\;\; = \;\;
\dfrac{1}{n}\sum_{i=1}^{n}\log\left(\,Y_{i}\,\right)
\;\; = \;\;
\dfrac{1}{n}\sum_{i=1}^{n}X_{i}
\;\; = \;\;
\overline{X}_{n}
\;\; \sim \;\;
N\!\left(\,\mu\,,\,\dfrac{\sigma^{2}}{n}\,\right)
\end{equation*}
Thus,
\begin{equation*}
\overline{Y}_{g}
\;\; = \;\;
e^{\overline{X}_{n}}
\;\; = \;\;
\textnormal{LogNormal}\!\left(\,\mu\,,\,\dfrac{\sigma^{2}}{n}\,\right)
\end{equation*}
Hence,
\begin{equation*}
E\!\left[\,\overline{Y}_{g}\,\right]
\;\;=\;\;
\exp\left\{\,\mu+\frac{\sigma^{2}}{2n}\,\right\}
\quad\textnormal{and}\quad
V\!\left[\,\overline{Y}_{g}\,\right]
\;\; = \;\;
\left[\,e^{\mu+\frac{\sigma^{2}}{2n}}\,\right]^{2}
\cdot
\left(e^{\frac{\sigma^{2}}{n}} - 1\right)
\;\; = \;\;
\left[\,e^{2\mu+\frac{\sigma^{2}}{n}}\,\right]
\cdot
\left(e^{\frac{\sigma^{2}}{n}} - 1\right)
\end{equation*}
Next,
\begin{equation*}
\textnormal{Cov}\left(\,\overline{Y_{a}}\,,\,\overline{Y}_{g}\,\right)
\;\;=\;\;
\textnormal{Cov}\left(\,
\dfrac{1}{n}\sum_{i=1}^{n}Y_{i}
\,,\,
\overline{Y}_{g}
\,\right)
\;\;=\;\;
\dfrac{1}{n}\sum_{i=1}^{n}
\textnormal{Cov}\left(\,
Y_{i}
\,,\,
\overline{Y}_{g}
\,\right)
\;\;=\;\;
\dfrac{1}{n}\sum_{i=1}^{n}
\left\{\,
E\!\left[\,Y_{i}\cdot \overline{Y}_{g}\,\right]
\;-\;
E\!\left[\,Y_{i}\,\right]\cdot E\!\left[\overline{Y}_{g}\,\right]
\,\right\}
\end{equation*}
Now,
\begin{eqnarray*}
          E\!\left[\,Y_{i}\cdot \overline{Y}_{g}\,\right]
&=&       E\!\left[\,Y_{i}\cdot \left(\,\prod_{k=1}^{n}Y_{k}\right)^{1/n} \,\right]
\;\;=\;\; E\!\left[\,Y_{i}\cdot \prod_{k=1}^{n}Y_{k}^{1/n} \,\right]
\;\;=\;\; E\!\left[\,Y_{i}^{1+\frac{1}{n}}\cdot \underset{k \neq i}{\prod_{k=1}^{n}}Y_{k}^{1/n} \,\right] \\
&=&       E\!\left[\,Y_{i}^{1+\frac{1}{n}}\,\right]
          \cdot
          E\!\left[\,\underset{k \neq i}{\prod_{k=1}^{n}}Y_{k}^{1/n} \,\right]
          \quad\textnormal{(by independence of $Y_{1},\ldots,Y_{n}$)} \\
\end{eqnarray*}
Now, note that
\begin{equation*}
\log\left(\,Y^{1+\frac{1}{n}}\,\right)
\;\;=\;\;
\left(1+\dfrac{1}{n}\right)\log(Y)
\;\;=\;\;
\left(1+\dfrac{1}{n}\right)X
\;\;\sim\;\;
N\!\left(\,\left(1+\dfrac{1}{n}\right)\mu\,,\,\left(1+\dfrac{1}{n}\right)^{2}\sigma^{2}\,\right)
\end{equation*}
Hence,
\begin{equation*}
Y^{1+\frac{1}{n}} \sim
\textnormal{LogNormal}
\!\left(\,\left(1+\dfrac{1}{n}\right)\mu\,,\,\left(1+\dfrac{1}{n}\right)^{2}\sigma^{2}\,\right)
\end{equation*}
and
\begin{equation*}
E\!\left[\,Y^{1+\frac{1}{n}}\,\right]
\;\; = \;\;
\exp\!\left\{\,
\left(1+\frac{1}{n}\right)\mu
\;+\;
\left(1+\frac{1}{n}\right)^{2}\dfrac{\sigma^{2}}{2}
\,\right\}
\end{equation*}
On the other hand,
\begin{equation*}
\log\!\left[\,\underset{k \neq i}{\prod_{k=1}^{n}}Y_{k}^{1/n} \,\right]
\;\;=\;\;
\log\!\left[\,\left(\,\underset{k \neq i}{\prod_{k=1}^{n}}Y_{k}\,\right)^{1/n} \,\right]
\;\;=\;\; \dfrac{1}{n} \underset{k\neq i}{\sum_{k=1}^{n}}\log Y_{k}
\;\;=\;\; \dfrac{1}{n} \underset{k\neq i}{\sum_{k=1}^{n}}X_{k}
\;\;\sim\;\;
N\!\left(\,\left(\dfrac{n-1}{n}\right)\mu\,,\,\left(\dfrac{n-1}{n^{2}}\right)\sigma^{2}\,\right)
\end{equation*}
Thus,
\begin{equation*}
\underset{k \neq i}{\prod_{k=1}^{n}}\,Y_{k}^{1/n}
\;\;\sim\;\;
\textnormal{LogNormal}
\!\left(\,\left(\dfrac{n-1}{n}\right)\mu\,,\,\left(\dfrac{n-1}{n^{2}}\right)\sigma^{2}\,\right)
\end{equation*}
Hence,
\begin{equation*}
E\!\left[\,\underset{k \neq i}{\prod_{k=1}^{n}}\,Y_{k}^{1/n}\,\right]
\;\;=\;\;
\exp
\!\left\{\,
\left(\dfrac{n-1}{n}\right)\mu\;+\;\left(\dfrac{n-1}{n^{2}}\right)\dfrac{\sigma^{2}}{2}
\,\right\}
\end{equation*}
Hence,
\begin{eqnarray*}
          \textnormal{Cov}\left(\, Y_{i} \,,\, \overline{Y}_{g} \,\right)
&=&       E\!\left[\,Y_{i}\cdot \overline{Y}_{g}\,\right]
          \;-\;
          E\!\left[\,Y_{i}\,\right]\cdot E\!\left[\overline{Y}_{g}\,\right]
\;\;=\;\; E\!\left[\,Y_{i}^{1+\frac{1}{n}}\,\right]
          \cdot
          E\!\left[\,\underset{k \neq i}{\prod_{k=1}^{n}}Y_{k}^{1/n} \,\right]
          \;-\;
          E\!\left[\,Y_{i}\,\right]\cdot E\!\left[\overline{Y}_{g}\,\right] \\
&=&       \exp\!\left\{
          \left(1+\frac{1}{n}\right)\mu
          \,+\,
          \left(1+\frac{1}{n}\right)^{2}\dfrac{\sigma^{2}}{2}
          \right\}
          \cdot
          \exp
          \!\left\{
          \left(\dfrac{n-1}{n}\right)\mu+\left(\dfrac{n-1}{n^{2}}\right)\dfrac{\sigma^{2}}{2}
          \right\}
          \; - \;
          \exp\left\{\mu + \frac{\sigma^{2}}{2} \right\}
          \exp\left\{\mu + \frac{\sigma^{2}}{2n}\right\} \\
&=&       \exp\!\left\{
          \left(1+\frac{1}{n}\right)\mu
          \,+\,
          \left(1+\frac{2}{n}+\dfrac{1}{n^{2}}\right)\dfrac{\sigma^{2}}{2}
          \,+\,
          \left(1-\dfrac{1}{n}\right)\mu+\left(\dfrac{1}{n}-\dfrac{1}{n^{2}}\right)\dfrac{\sigma^{2}}{2}
          \right\}
          \; - \;
          \exp\left\{2\mu + \frac{\sigma^{2}}{2}\left(1+\frac{1}{n}\right) \right\} \\
&=&       \exp\!\left\{
          2\mu \,+\,
          \dfrac{\sigma^{2}}{2}
          \left(1+\frac{3}{n}\right)
          \right\}
          \; - \;
          \exp\left\{2\mu + \frac{\sigma^{2}}{2}\left(1+\frac{1}{n}\right) \right\} \\
&=&       \exp\!\left\{
          2\mu \,+\,
          \dfrac{\sigma^{2}}{2}
          \left(1+\frac{1}{n}\right)
          \right\}
          \cdot
          \left\{\,\exp\left(\,\dfrac{\sigma^{2}}{n}\,\right)-1\,\right\} \\
\end{eqnarray*}
So,
\begin{eqnarray*}
          \textnormal{Cov}\left(\,\overline{Y_{a}}\,,\,\overline{Y}_{g}\,\right)
&=&       \textnormal{Cov}\left(\,
          \dfrac{1}{n}\sum_{i=1}^{n}Y_{i}
          \,,\,
          \overline{Y}_{g}
          \,\right)
\;\;=\;\; \dfrac{1}{n}\sum_{i=1}^{n}
          \textnormal{Cov}\left(\,
          Y_{i}
          \,,\,
          \overline{Y}_{g}
          \,\right)
\;\;=\;\; \dfrac{n}{n}\exp\!\left\{
          2\mu \,+\,
          \dfrac{\sigma^{2}}{2}
          \left(1+\frac{1}{n}\right)
          \right\}
          \cdot
          \left\{\,\exp\left(\,\dfrac{\sigma^{2}}{n}\,\right)-1\,\right\} \\
\\
&=&       \exp\!\left\{
          2\mu \,+\,
          \dfrac{\sigma^{2}}{2}
          \left(1+\frac{1}{n}\right)
          \right\}
          \cdot
          \left\{\,\exp\left(\,\dfrac{\sigma^{2}}{n}\,\right)-1\,\right\} \\
\end{eqnarray*}
Lastly,
\begin{eqnarray*}
          \textnormal{Corr}\left(\,\overline{Y_{a}}\,,\,\overline{Y}_{g}\,\right)
&=&       \dfrac{\textnormal{Cov}\left(\,\overline{Y_{a}}\,,\,\overline{Y}_{g}\,\right)}
          {\sqrt{V\!\left[\,\overline{Y}_{a}\,\right]\cdot V\!\left[\,\overline{Y}_{g}\,\right]}}
\\
&=&       \dfrac{
          \exp\!\left\{
          2\mu \,+\,
          \dfrac{\sigma^{2}}{2}
          \left(1+\frac{1}{n}\right)
          \right\}
          \cdot
          \left\{\,\exp\left(\,\dfrac{\sigma^{2}}{n}\,\right)-1\,\right\}
          }{
          \sqrt{
          \dfrac{1}{n}\left(e^{2\mu+\sigma^{2}}\right)\cdot\left(e^{\sigma^{2}}-1\right)
          \cdot
          \left(\,e^{2\mu+\frac{\sigma^{2}}{n}}\,\right)
          \cdot
          \left(e^{\frac{\sigma^{2}}{n}} - 1\right)
          }
          }
\\
&=&       \dfrac{
          \sqrt{n}\cdot
          \exp\!\left\{
          2\mu \,+\,
          \dfrac{\sigma^{2}}{2}
          \left(1+\frac{1}{n}\right)
          \right\}
          \cdot
          \left\{\,\exp\left(\,\dfrac{\sigma^{2}}{n}\,\right)-1\,\right\}
          }{
          \left(e^{\mu+\frac{\sigma^{2}}{2}}\right)
          \cdot
          \sqrt{e^{\sigma^{2}}-1}
          \cdot
          \left(\,e^{\mu+\frac{\sigma^{2}}{2n}}\,\right)
          \cdot
          \sqrt{e^{\frac{\sigma^{2}}{n}} - 1}
          }
\\
&=&       \dfrac{
          \sqrt{n}\cdot\left\{\,\exp\left(\,\dfrac{\sigma^{2}}{n}\,\right)-1\,\right\}
          }{
          \sqrt{e^{\sigma^{2}}-1}
          \cdot
          \sqrt{e^{\frac{\sigma^{2}}{n}} - 1}
          }
\\
&=&       \sqrt{\dfrac{
          n\cdot
          \left(\,e^{\frac{\sigma^{2}}{n}}-1\,\right)
          }{
          e^{\sigma^{2}}-1
          }}
\\
\end{eqnarray*}

%%%%%%%%%%%%%%%%%%%%%%%%%%%%%%%%%%%%%%%%%%%%%%%%%%%%%%%%%%%%%%%%%%%%%%%%%%%%%%%%%%%%%%%%%%%%%%%%%%%%

