
\noindent
\textbf{Exercise 3.14}

\vskip 0.3cm
\noindent
\textbf{Solution 1 (without using moment generating functions)}

\vskip 0.3cm
\noindent
First, note that for $k = 0, 1, 2, \ldots$, we have:
\begin{eqnarray*}
          P(\,Y_{p} = k\,)
&=&       \sum_{y=0}^{\infty}\,P(\,Y_{p} = k\,\vert\,Y=y\,)\cdot P(Y = y)
\;\;=\;\; \sum_{y=k}^{\infty}\,P(\,Y_{p} = k\,\vert\,Y=y\,)\cdot P(Y = y)
\\
&=&       \sum_{y=k}^{\infty}
          \left(\!\begin{array}{c} y \\ k \end{array}\!\right)
          \pi^{k} (1 - \pi)^{y-k} \cdot e^{-\lambda L} \dfrac{(\lambda L)^{y}}{y!}
\\
&=&
          e^{-\lambda L}\,\left(\dfrac{\pi}{1-\pi}\right)^{k}\cdot
          \sum_{y=k}^{\infty}\,
          \dfrac{y!}{k!\,(y-k)!}\cdot\dfrac{((1-\pi)\lambda L)^{y}}{y!}
\\
&=&
          e^{-\lambda L}\,\left(\dfrac{\pi}{1-\pi}\right)^{k}\dfrac{1}{k!}
          \cdot
          \sum_{y=k}^{\infty}\,\dfrac{((1-\pi)\lambda L)^{y}}{(y-k)!}
\\
&=&
          e^{-\lambda L}\,\left(\dfrac{\pi}{1-\pi}\right)^{k}\dfrac{1}{k!}
          \cdot
          \sum_{m=0}^{\infty}\,\dfrac{((1-\pi)\lambda L)^{m+k}}{m!}
\\
&=&
          e^{-\lambda L}\,\left(\dfrac{\pi}{1-\pi}\right)^{k}\dfrac{1}{k!}
          \cdot
          ((1-\pi)\lambda L)^{k}
          \cdot
          \sum_{m=0}^{\infty}\,\dfrac{((1-\pi)\lambda L)^{m}}{m!}
\\
&=&
          e^{-\lambda L}\,\left(\dfrac{\pi}{1-\pi}\right)^{k}\dfrac{1}{k!}
          \cdot
          ((1-\pi)\lambda L)^{k}
          \cdot e^{(1-\pi)\lambda L}
\\
&=&       e^{-\lambda L+\lambda L - \pi\lambda L}\,\dfrac{\left(\pi\lambda L\right)^{k}}{k!}
\\
&=&       e^{-\pi\lambda L}\,\dfrac{\left(\pi\lambda L\right)^{k}}{k!}
\end{eqnarray*}
Thus, we see that $Y_{p} \sim \textnormal{Poisson}(\pi\lambda L)$.

%%%%%%%%%%%%%%%%%%%%%%%%%%%%%%%%%%%%%%%%%%%%%%%%%%%%%%%%%%%%%%%%%%%%%%%%%%%%%%%%%%%%%%%%%%%%%%%%%%%%

