
%%%%%%%%%%

\newcommand{\modelParameters}{
	\begin{array}{c}
		\pi_{c \vert x}\,, \; \mu_{m \vert xy}\,, \; \nu_{xy}\,, \; \omega_{j}
		\\
		\textnormal{$c,y\in\{0,1\}, \, x\in\{0,1\}^{p},$}
		\\
		\textnormal{$m,j\in\{0,1\}$}
	\end{array}
}

\newcommand{\EMConditions}{
	\begin{array}{c}
		X^{(a)},\,\widetilde{Y}^{(a)},\,K^{(a)}
		\\
		\textnormal{$a\in\{1,\ldots,n\}$}
	\end{array}
	\textnormal{\large;}
	\modelParameters
}

\newcommand{\EMConditionsWithValues}{
	\begin{array}{c}
		X^{(a)} = x^{(a)} ,\, \widetilde{Y}^{(a)} = y_{a} ,\, K^{(a)} = k_{a}
		\\
		\textnormal{$a\in\{1,\ldots,n\}$}
	\end{array}
	\textnormal{\large;}
	\modelParameters
}

\newcommand{\ithEMConditionsWithValues}{
	\begin{array}{c}
		X^{(i)} = x^{(i)} ,\, \widetilde{Y}^{(i)}=y_{i} ,\, K^{(i)}=k_{i}
	\end{array}
	\textnormal{\large;}
	\modelParameters
}

\newcommand{\ithGYZeroEMConditionsWithValues}{
	\begin{array}{c}
		X^{(i)}=x , \widetilde{Y}^{(i)}=y , K^{(i)}=0
	\end{array}
	\textnormal{\large;}
	\modelParameters
}

\newcommand{\ithGYOneEMConditionsWithValues}{
	\begin{array}{c}
		X^{(i)}=x , \widetilde{Y}^{(i)}=y , K^{(i)}=1
	\end{array}
	\textnormal{\large;}
	\modelParameters
}

\newcommand{\ithGYTwoEMConditionsWithValues}{
	\begin{array}{c}
		X^{(i)}=x , \widetilde{Y}^{(i)}=y , K^{(i)}=2
	\end{array}
	\textnormal{\large;}
	\modelParameters
}

\newcommand{\logisticBetaX}{
	\dfrac{\exp\!\left(\,\beta^{T} \cdot x \,\right)}{1 \,+\, \exp\!\left(\,\beta^{T} \cdot x \,\right)}
}

\newcommand{\oneMinusLogisticBetaX}{
	\dfrac{1}{1 \,+\, \exp\!\left(\,\beta^{T} \cdot x \,\right)}
}

%%%%%%%%%%

\begin{frame}{\Large The random variables involved ...}

\scriptsize
\begin{center}
\begin{tabular}{|c|c|l|}
\hline
$\overset{{\color{white}.}}{X^{(i)}}$ & observed & multivariate predictor variable with binary component variables
\\ \hline
$\overset{{\color{white}.}}{Y^{(i)}}$ & unobserved & (true) binary response variable
\\ \hline
$\overset{{\color{white}.}}{\widetilde{Y}^{(i)}}$ & observed & observed binary response variable (may contain measurement errors)
\\ \hline
$M^{(i)}$ & $\begin{array}{c} \textnormal{partially} \\ \textnormal{observed} \end{array}$ &
	\!\!\!$\begin{array}{l}
		{\color{white}.}
		\\
		\textnormal{binary variable indicating whether clerical review}
		\\
		\textnormal{confirms correctness of \,$\overset{{\color{white}.}}{\widetilde{Y}^{(i)}}$}
		\\
		{\color{white}.}
	\end{array}$ 
\\ \hline
$\overset{{\color{white}.}}{J^{(i)}}$ & $\begin{array}{c} \textnormal{partially} \\ \textnormal{observed} \end{array}$ &
	\!\!\!$\begin{array}{l}
		{\color{white}.}
		\\
		\textnormal{binary variable indicating whether}
		\\
		\textnormal{observation $i$ is selected for clerical review}
		\\
		{\color{white}.}
	\end{array}$
\\ \hline
&& \\
$K^{(i)}$ & observed & $K^{(i)} \;:=\;
	\left\{\begin{array}{cl}
		0, & \textnormal{if}\;\; J^{(i)} = 0,
		\\
		1, & \textnormal{if}\;\; J^{(i)} = 1, \;\;\textnormal{and}\;\; M^{(i)} = 0,
		\\
		2, & \textnormal{if}\;\; J^{(i)} = 1, \;\;\textnormal{and}\;\; M^{(i)} = 1
	\end{array}\right.$
\\
&& \\
\hline
\end{tabular}
\end{center}

\end{frame}
\normalsize

%%%%%%%%%%

\begin{frame}{\Large Want to prove ...}

\small
The logarithm of the joint probability distribution of
\begin{equation*}
Y^{(i)}\,, X^{(i)}\,, \widetilde{Y}^{(i)}\,, K^{(i)}\,,
\quad
\textnormal{for \;$i \in \{1,2,\ldots,n\}$}\,,
\end{equation*}
is given by:
\scriptsize
\begin{eqnarray*}
	&&
		\log\,L
	\\
		&=&
		\log\,P\!\left(\;
			\overset{n}{\underset{i=1}{\bigcap}}\;
			\left\{
				Y^{(i)}=c_{i},X^{(i)}=x^{(i)},\widetilde{Y}^{(i)}=y_{i},K^{(i)}=k_{i}
			\right\}
		\;\right)
	\\
	&=&
		{\color{white}+} \;\;
		\overset{1}{\underset{c=0}{\sum}}\;\;
		\underset{x\in\{0,1\}^{p}}{\sum}\;\;
		\overset{1}{\underset{y=0}{\sum}}\;
		\left(\overset{n}{\underset{i=1}{\sum}}\;W^{(i)}_{c \vert xy{\color{red}0}}\right)
		\cdot
		\left(\,
			\log\left(\pi_{c \vert x}\,\mu_{0 \vert xy} + \delta_{cy}\,\mu_{1\vert xy}\right)
			\,\overset{{\color{white}.}}{+}\,
			\log\,\nu_{xy}
			\,\overset{{\color{white}.}}{+}\,
			\log\,\omega_{0}
		\,\right)
	\\
	&&
		+ \;\;
		\overset{1}{\underset{c=0}{\sum}}\;\;
		\underset{x\in\{0,1\}^{p}}{\sum}\;\;
		\overset{1}{\underset{y=0}{\sum}}\;
		\left(\overset{n}{\underset{i=1}{\sum}}\;W^{(i)}_{c \vert xy{\color{red}1}}\right)
		\cdot
		\left(\,
			\log\,\pi_{c \vert x}
			\,\overset{{\color{white}.}}{+}\,
			\log\,\mu_{0\vert xy}
			\,\overset{{\color{white}.}}{+}\,
			\log\,\nu_{xy}
			\,\overset{{\color{white}.}}{+}\,
			\log\,\omega_{1}
		\,\right)
	\\
	&&
		+ \;\;
		\overset{1}{\underset{y=0}{\sum}}\;\;
		\underset{x\in\{0,1\}^{p}}{\sum}\,
		\left(\overset{n}{\underset{i=1}{\sum}}\;W^{(i)}_{y \vert xy{\color{red}2}}\right)
		\cdot
		\left(\,
			\log\,\mu_{1 \vert xy}
			\,\overset{{\color{white}.}}{+}\,
			\log\,\nu_{xy}
			\,\overset{{\color{white}.}}{+}\,
			\log\,\omega_{1}
		\,\right)
\end{eqnarray*}

\end{frame}
\normalsize

%%%%%%%%%%

\begin{frame}{\Large The quantities involved ...}

\normalsize
\begin{equation*}
\begin{array}{ccll}
	W^{(i)}_{c \vert xyk}
		&:=&
		\overset{\textnormal{\large\color{white}1}}{I}\!\left\{\,Y^{(i)}=c,X^{(i)}=x,\widetilde{Y}^{(i)}=y,K^{(i)}=k\,\right\}
	\\
	{\color{red}\pi_{c \vert x}}
		&\overset{{\color{white}\vert}}{:=}&
		P\!\left(\,\left.\overset{{\color{white}.}}{Y}=c\;\right\vert X=x\,\right)
	\\
	\mu_{m \vert xy}
		&\overset{{\color{white}\vert}}{:=}&
		P\!\left(\,\left.\overset{{\color{white}.}}{M}=m\;\right\vert X=x, \widetilde{Y}=y\,\right)
	\\
	\nu_{xy}
		&\overset{{\color{white}\vert}}{:=}&
		P\!\left(\,\overset{{\color{white}.}}{X}=x, \widetilde{Y}=y\,\right)
	\\
	\omega_{j}
		&\overset{{\color{white}\vert}}{:=}&
		P\!\left(\,\overset{{\color{white}.}}{J}=j\,\right)
	\\
	\overset{\textnormal{\Large\color{white}1}}{\delta}_{cy}
		&\overset{{\color{white}\vert}}{:=}&
		\left\{\begin{array}{cl}
			1, & \textnormal{if}\;\; c = y\,,
			\\
			0, & \textnormal{otherwise}\,.
		\end{array}\right.
\end{array}
\end{equation*}

\end{frame}
\normalsize

%%%%%%%%%%

\begin{frame}{\vskip -0.25cm \Large Assumptions ...}

\tiny

\renewcommand{\theenumi}{\alph{enumi}}
\begin{enumerate}
\item
	There exists $\beta \in \Re^{p}$ such that
	\begin{equation*}
	\pi_{1 \vert x}
	\;\; := \;\;
		P\!\left(\; Y^{(i)} = 1 \,\left\vert\, X^{(i)} = x \right.\,\right)
	\;\; = \;\;
		E\!\left[\; Y^{(i)}  = 1 \,\left\vert\, X^{(i)} = x \right.\,\right]
	\;\; = \;\;
		\logisticBetaX\,,
	\quad
	\end{equation*}
	for each $x \in \{0,1\}^{p}$ and for each \,$i = 1,2,\ldots,n$.
\item\label{iIndependence}
	The $\left(\left\{0,1\right\} \overset{{\color{white}.}}{\times} \left\{0,1\right\}^{p} \times \left\{0,1\right\} \times \left\{0,1\right\}\right)$-valued
	random variables
	\,$Z^{(i)} := \left(\,Y^{(i)},X^{(i)},\widetilde{Y}^{(i)},M^{(i)}\,\right)$,
	\,$i \in \{1, \ldots, n\}$,
	\,are independent and identically distributed.
\item\label{Jindependence}
	The Bernoulli random variables \,$J^{(i)}$, \,$i \in \{1, \ldots, n\}$, \,are independent and identically distributed.
\item\label{ZJindependence}
	The two collections of random variables
	\,$\left\{\,Z^{(i)} := \left(\,Y^{(i)},X^{(i)},\widetilde{Y}^{(i)},M^{(i)}\right)\,\right\}_{i=1}^{n}$\,
	and
	\,$\left\{\,J^{(i)}\,\right\}_{i=1}^{n}$\,
	are independent, in the sense that, for all
	\,$z_{1}, \ldots, z_{n} \in \left\{0,1\right\}^{p+3}$\, and \,$j_{1}, \ldots, j_{n} \in \{0,1\}$,\,
	\begin{eqnarray*}
	&&
		P\!\left(\,Z^{(1)}=z_{1},\,\ldots\,,Z^{(n)}=z_{n},\;J^{(1)}=j_{1},\,\ldots\,,J^{(n)}=j_{n}\,\right)
	\\
	& = &
		P\!\left(\,Z^{(1)}=z_{1},\,\ldots\,,Z^{(n)}=z_{n}\,\right)
		\cdot
		P\!\left(\,J^{(1)}=j_{1},\,\ldots\,,J^{(n)}=j_{n}\,\right)
	\end{eqnarray*}
\item\label{MzeroImplies}
	{\color{red}For each \,$i\in\{1,2,\ldots,n\}$, \,$c\in\{0,1\}$, \,$x \in \{0,1\}^{p+3}$, and \,$y \in \{0,1\}$, \,we have:
	\begin{equation*}
	P\!\left(\left.Y^{(i)} = c\,\;\right\vert X^{(i)}=x,\widetilde{Y}^{(i)}=y,M^{(i)}=0\,\right)
	\;\; = \;\;
	P\!\left(\;Y^{(i)} = c\;\left\vert\,X^{(i)}=x\right.\,\right)\,.
	\end{equation*}}
\item\label{MoneImpliesCEqualsY}
	For each $i\in\{1,2,\ldots,n\}$, we have:
	\begin{equation*}
	M^{(i)} \; = \; 1
	\quad\Longrightarrow\quad
	Y^{(i)} \; = \; \widetilde{Y}^{(i)},
	\end{equation*}
	which, in particular, implies $P\!\left(\,\left.Y^{(i)} = \widetilde{Y}^{(i)}\;\right\vert\;M^{(i)}=1\,\right)\,=\,1$.
\end{enumerate}

\end{frame}
\normalsize

%%%%%%%%%%

\begin{frame}{\vskip -0.20cm\Large Proof ...}

\vskip -0.5cm

\scriptsize
\begin{eqnarray*}
L &=&
	P\!\left(\;
		\overset{n}{\underset{i=1}{\bigcap}}\;
		\left\{
			Y^{(i)}=c_{i},X^{(i)}=x^{(i)},\widetilde{Y}^{(i)}=y_{i},K^{(i)}=k_{i}
		\right\}
	\;\right)
\\
\pause
&=&
	\overset{n}{\underset{i=1}{\prod}} \;\,
	P\!\left(\,Y^{(i)}=c_{i},X^{(i)}=x^{(i)},\widetilde{Y}^{(i)}=y_{i},K^{(i)}=k_{i}\,\right)
\\
\pause
&=&
	\overset{n}{\underset{i=1}{\prod}} \;
	\left\{\;
		\overset{1}{\underset{c=0}{\prod}}
		\,\;\underset{x\in\{0,1\}^{p}}{\prod}\;\,
		\overset{1}{\underset{y=0}{\prod}}\;\;
		\overset{2}{\underset{k=0}{\prod}}\;\;
		P\!\left(\,Y=c,X=x,\widetilde{Y}=y,K=k\,\right)^{W^{(i)}_{c \vert xyk}}
	\;\right\}
\\
\pause
&=&
	\overset{1}{\underset{c=0}{\prod}}
	\,\;\underset{x\in\{0,1\}^{p}}{\prod}\;\,
	\overset{1}{\underset{y=0}{\prod}}\;\;
	\overset{2}{\underset{k=0}{\prod}}\;
	\left\{\;
		\overset{n}{\underset{i=1}{\prod}} \;\,
		P\!\left(\,Y=c,X=x,\widetilde{Y}=y,K=k\,\right)^{W^{(i)}_{c \vert xyk}}
	\;\right\}
\\
\pause
&=&
	\overset{1}{\underset{c=0}{\prod}}
	\,\;\underset{x\in\{0,1\}^{p}}{\prod}\;\,
	\overset{1}{\underset{y=0}{\prod}}\;\;
	\overset{2}{\underset{k=0}{\prod}}\;
	\left\{\;
		P\!\left(\,Y=c,X=x,\widetilde{Y}=y,K=k\,\right)
		^{\overset{n}{\underset{i=1}{\sum}}\,W^{(i)}_{c \vert xyk}}
	\;\right\}\,.
\end{eqnarray*}

\vskip -0.40cm

\pause
\begin{eqnarray*}
\log\,L &=&
	\overset{1}{\underset{c=0}{\sum}}
	\,\;\underset{x\in\{0,1\}^{p}}{\sum}\;\,
	\overset{1}{\underset{y=0}{\sum}}\;\;
	\overset{2}{\underset{k=0}{\sum}}\;
	\left(\overset{n}{\underset{i=1}{\sum}}\;W^{(i)}_{c \vert xyk}\right)
	\cdot
	\log\,P\!\left(\,Y=c,X=x,\widetilde{Y}=y,K=k\,\right)
\end{eqnarray*}

\end{frame}
\normalsize

%%%%%%%%%%

\begin{frame}{\vskip -0.20cm\Large Proof ...}

\tiny
\begin{eqnarray*}
\log\,L &=&
	\overset{1}{\underset{c=0}{\sum}}
	\,\;\underset{x\in\{0,1\}^{p}}{\sum}\;\,
	\overset{1}{\underset{y=0}{\sum}}\;\;
	\overset{2}{\underset{k=0}{\sum}}\;
	\left(\overset{n}{\underset{i=1}{\sum}}\;W^{(i)}_{c \vert xyk}\right)
	\cdot
	\log\,P\!\left(\,Y=c,X=x,\widetilde{Y}=y,K=k\,\right)
\\
\pause
&=&
	\overset{1}{\underset{c=0}{\sum}}
	\,\;\underset{x\in\{0,1\}^{p}}{\sum}\;\,
	\overset{1}{\underset{y=0}{\sum}}\;\;
	\overset{2}{\underset{k=0}{\sum}}\;
	\left(\overset{n}{\underset{i=1}{\sum}}\;W^{(i)}_{c \vert xyk}\right)
	\cdot
	\log\left[\,
		\begin{array}{c}
			P\!\left(\,Y=c\,\left\vert\,X=x,\widetilde{Y}=y,K=k\right.\,\right)
			\\
			\times \; P\!\left(\,X=x,\widetilde{Y}=y,K=k\,\right)
		\end{array}
	\,\right]
\\
\pause
&=&
	\overset{1}{\underset{c=0}{\sum}}
	\,\;\underset{x\in\{0,1\}^{p}}{\sum}\;\,
	\overset{1}{\underset{y=0}{\sum}}\;\;
	\overset{2}{\underset{k=0}{\sum}}\;
	\left(\overset{n}{\underset{i=1}{\sum}}\;W^{(i)}_{c \vert xyk}\right)
	\cdot
	\log\left[\,
		\pi_{c \vert xyk} \overset{{\color{white}\vert}}{\cdot} p_{xyk}
	\,\right]
\\
\pause
&=&
	{\color{white}+} \;\;
	\overset{1}{\underset{c=0}{\sum}}
	\,\;\underset{x\in\{0,1\}^{p}}{\sum}\;\,
	\overset{1}{\underset{y=0}{\sum}}\;
	\left(\overset{n}{\underset{i=1}{\sum}}\;W^{(i)}_{c \vert xy{\color{red}0}}\right)
	\cdot
	\log\left[\,
		\pi_{c \vert xy\color{red}0} \cdot p_{xy\color{red}0}
	\,\right]
\\
&&
	+ \;\;
	\overset{1}{\underset{c=0}{\sum}}
	\,\;\underset{x\in\{0,1\}^{p}}{\sum}\;\,
	\overset{1}{\underset{y=0}{\sum}}\;
	\left(\overset{n}{\underset{i=1}{\sum}}\;W^{(i)}_{c \vert xy{\color{red}1}}\right)
	\cdot
	\log\left[\,
		\pi_{c \vert xy\color{red}1} \cdot p_{xy\color{red}1}
	\,\right]
\\
&&
	+ \;\;
	\overset{1}{\underset{y=0}{\sum}}\;
	\,\;\underset{x\in\{0,1\}^{p}}{\sum}\,
	\left(\overset{n}{\underset{i=1}{\sum}}\;W^{(i)}_{y \vert xy{\color{red}2}}\right)
	\cdot
	\log\left[\,
		\pi_{y \vert xy\color{red}2} \cdot p_{xy\color{red}2}
	\,\right]
\end{eqnarray*}

\pause
\begin{eqnarray*}
W^{(i)}_{c \vert xy{\color{red}2}}
&:=&
	I\!\left\{\,Y^{(i)}=c,X^{(i)}=x,\widetilde{Y}^{(i)}=y,K^{(i)}={\color{red}2}\,\right\}
\\
&=&
	I\!\left\{\,Y^{(i)}=c,X^{(i)}=x,\widetilde{Y}^{(i)}=y,J^{(i)}=1,M^{(i)}=1\,\right\}
%\\
%&=&
\;\; = \;\;
	\left\{\begin{array}{cl}
		1, & \textnormal{if}\;\; c = y
		\\
		0, & \textnormal{otherwise}
	\end{array}\right.
\end{eqnarray*}

\end{frame}
\normalsize

%%%%%%%%%%

\begin{frame}{\vskip -0.20cm\Large Proof ...}

\scriptsize

\begin{eqnarray*}
\pi_{c \vert xy0}
\pause
&=&
	P\!\left(\;Y=c\;\left\vert\;X=x,\widetilde{Y}=y,K=0\right.\,\right)
\\
\pause
&=&
	P\!\left(\;Y=c\;\left\vert\;X=x,\widetilde{Y}=y,J=0\right.\,\right)
\\
\pause
&=&
	P\!\left(\;Y=c\;\left\vert\;X=x,\widetilde{Y}=y\right.\,\right),
	\quad\quad
	\textnormal{by \eqref{ZJindependence}}
\\
\pause
&=&
	P\!\left(\;Y=c,M=0\;\left\vert\;X=x,\widetilde{Y}=y\right.\,\right)
	\;+\;
	P\!\left(\;Y=c,M=1\;\left\vert\;X=x,\widetilde{Y}=y\right.\,\right)
\\
\pause
&=&
	{\color{white}+}\;\;
	P\!\left(\;Y=c\;\left\vert\;M=0,X=x,\widetilde{Y}=y\right.\,\right)
	\cdot
	P\!\left(\;M=0\;\left\vert\;X=x,\widetilde{Y}=y\right.\,\right)
\\
\pause
&&
	+\;\;
	P\!\left(\;Y=c\;\left\vert\;M=1,X=x,\widetilde{Y}=y\right.\,\right)
	\cdot
	P\!\left(\;M=1\;\left\vert\;X=x,\widetilde{Y}=y\right.\,\right)
\\
\pause
&=&
	P\!\left(\;\left.Y\overset{{\color{white}-}}{=}c\;\right\vert X=x\;\right)
	\cdot
	\mu_{0 \vert xy}
	\;\;+\;\;
	\delta_{cy}
	\cdot
	\mu_{1 \vert xy}\,,
	\quad\;
	\textnormal{by \,\eqref{MzeroImplies}, \eqref{MoneImpliesCEqualsY},\, and definition of \,$\mu_{m \vert xy}$}
\\
\pause
&=&
	\pi_{c \vert x}
	\cdot
	\mu_{0 \vert xy}
	\;\;+\;\;
	\delta_{cy}
	\cdot
	\mu_{1 \vert xy}\,,
	\quad\quad
	\textnormal{by definition of \,$\pi_{c \vert x}$}
\end{eqnarray*}

\end{frame}
\normalsize

%%%%%%%%%%

\begin{frame}{\vskip -0.20cm\Large Proof ...}

\vskip -0.20cm

\small

\begin{eqnarray*}
\pi_{c \vert xy1}
&=&
	P\!\left(\;Y=c\;\left\vert\;X=x,\widetilde{Y}=y,K=1\right.\,\right)
\\
&=&
	P\!\left(\;Y=c\;\left\vert\;X=x,\widetilde{Y}=y,J=1,M=0\right.\,\right)
\\
&=&
	P\!\left(\;Y=c\;\left\vert\;X=x,\widetilde{Y}=y,M=0\right.\,\right),
	\quad\quad
	\textnormal{by \eqref{ZJindependence}}
\\
&=&
	P\!\left(\;Y=c\;\left\vert\;X\overset{{\color{white}-}}{=}x\right.\,\right),
	\quad\quad
	\textnormal{by \,\eqref{MzeroImplies}}
\\
&=&
	\pi_{c \vert x}\,,
	\quad\quad
	\textnormal{by definition of \,$\pi_{c \vert x}$}
\end{eqnarray*}

\begin{eqnarray*}
\pi_{y \vert xy2}
&=&
	P\!\left(\;Y=y\;\left\vert\;X=x,\widetilde{Y}=y,K=2\right.\,\right)
\\
&=&
	P\!\left(\;Y=y\;\left\vert\;X=x,\widetilde{Y}=y,J=1,M=1\right.\,\right)
\\
&=&
	1\,,
	\quad\quad
	\textnormal{by \eqref{MoneImpliesCEqualsY}.}
\end{eqnarray*}

\end{frame}
\normalsize

%%%%%%%%%%

\begin{frame}{\vskip -0.20cm\Large Also want to show:}

\tiny

	\begin{eqnarray*}
	E\!\left[\;\,
		\left.
		\overset{n}{\underset{i=1}{\sum}}\;W^{(i)}_{c \vert xy{\color{red}0}}
		\,\;\right\vert
		\EMConditions
	\right]
		&=&
		N_{xy{\color{red}0}}\cdot\left(\,\pi_{c \vert x}\,\mu_{0 \vert xy} \,+\, \delta_{cy}\,\mu_{1 \vert xy}\,\right)
	\\ \\
	E\!\left[\;\,
		\left.
		\overset{n}{\underset{i=1}{\sum}}\;W^{(i)}_{c \vert xy{\color{red}1}}
		\,\;\right\vert
		\EMConditions
	\right]
		&=&
		N_{xy{\color{red}1}}\cdot\pi_{c \vert x}
	\\ \\
	E\!\left[\;\,
		\left.
		\overset{n}{\underset{i=1}{\sum}}\;W^{(i)}_{c \vert xy{\color{red}2}}
		\,\;\right\vert
		\EMConditions
	\right]
		&=&
		N_{xy{\color{red}2}}\,,
	\end{eqnarray*}
	where \;$N_{xy{\color{red}k}}$ $:=$
	$\overset{n}{\underset{i=1}{\sum}}\,I\!\left\{\,X^{(i)}=x,\,\widetilde{Y}^{(i)}=y,\,K^{(i)}={\color{red}k}\,\right\}$,
	for $k \in \{0,1,2\}$.

\end{frame}
\normalsize

%%%%%%%%%%

\begin{frame}{\vskip -0.20cm\Large Proof ...}

\tiny

	\begin{eqnarray*}
	&&
		E\!\left[\;
			\left.
			W^{(i)}_{c \vert xy{\color{red}0}}
			\,\;\right\vert
			\EMConditionsWithValues
		\right]
	\\
	&=&
		E\!\left[\;
			\left.
			W^{(i)}_{c \vert xy{\color{red}0}}
			\,\;\right\vert
			\ithEMConditionsWithValues
		\right]\,,
		\quad
		\textnormal{by \; \eqref{iIndependence}, \eqref{Jindependence} and \eqref{ZJindependence}.}
	\\
	&=&
		P\!\left(\,
			\left.
			W^{(i)}_{c \vert xy{\color{red}0}} = 1
			\,\;\right\vert
			\ithEMConditionsWithValues
		\right)
	\\
	&=&
		P\!\left(\,
			\left.
			Y^{(i)} = c, X^{(i)} = x, \widetilde{Y}^{(i)} = y, K^{(i)} = 0
			\,\;\right\vert
			\!\!
			\ithEMConditionsWithValues
		\!\!\right)
	\\
	&=&
		I\!\left\{\,X^{(i)}=x , \widetilde{Y}^{(i)}=y , K^{(i)}\,=0\,\right\}
		\cdot
		P\!\left(
			\left.
			Y^{(i)} = c
			\,\;\right\vert
			\!\!
			\ithGYZeroEMConditionsWithValues
		\!\!\right)
	\\
	&=&
		I^{(i)}_{xy0}
		\cdot
		P\!\left(
			\left.
			Y^{(i)} = c
			\,\;\right\vert
			\!\!
			\begin{array}{c}
				X^{(i)} = x,\, \widetilde{Y}^{(i)} = y,\, J^{(i)} = 0
			\end{array}
			\textnormal{\large;}
			\modelParameters
		\!\!\right)
	\\
	&=&
		I^{(i)}_{xy0}
		\cdot
		P\!\left(
			\left.
			Y^{(i)} = c
			\,\;\right\vert
			\!\!
			\begin{array}{c}
				X^{(i)} = x,\, \widetilde{Y}^{(i)} = y
			\end{array}
			\textnormal{\large;}
			\;\;\cdots\;\;
		\right)\,,
		\quad
		\textnormal{by \eqref{ZJindependence} and suppressing parameters for brevity}
%	\\
%	&=&
%		I^{(i)}_{xy0}
%		\cdot
%		\left\{\;
%			P\!\left(\,
%				\left.
%				Y^{(i)} = c,\,M^{(i)}=0
%				\;\right\vert
%				X^{(i)} = x,\, \widetilde{Y}^{(i)} = y
%			\;\right)
%			\;+\;
%			P\!\left(\,
%				\left.
%				Y^{(i)} = c,\,M^{(i)}=1
%				\;\right\vert
%				X^{(i)} = x,\, \widetilde{Y}^{(i)} = y
%			\;\right)
%		\;\right\}
%	\\
%	&=&
%		I^{(i)}_{xy0}
%		\cdot
%		\left\{\;
%		\begin{array}{cc}
%			&
%			P\!\left(\,
%				\left.
%				Y^{(i)} = c
%				\;\right\vert
%				M^{(i)}=0,\,X^{(i)} = x,\, \widetilde{Y}^{(i)} = y
%			\;\right)
%			\cdot
%			P\!\left(\,
%				\left.
%				M^{(i)}=0
%				\;\right\vert
%				X^{(i)} = x,\, \widetilde{Y}^{(i)} = y
%			\;\right)
%		\\
%			\overset{\textnormal{\large{\color{white}1}}}{+}&
%			P\!\left(\,
%				\left.
%				Y^{(i)} = c
%				\;\right\vert
%				M^{(i)}=1,\, X^{(i)} = x,\, \widetilde{Y}^{(i)} = y
%			\;\right)
%			\cdot
%			P\!\left(\,
%				\left.
%				M^{(i)}=1
%				\;\right\vert
%				X^{(i)} = x,\, \widetilde{Y}^{(i)} = y
%			\;\right)
%		\end{array}
%		\;\right\}
%	\\
%	&=&
%		I^{(i)}_{xy0}
%		\cdot
%		\left(\;
%			\pi_{c \vert xy}
%			\cdot
%			\mu_{0 \vert xy}
%			\;\overset{{\color{white}.}}{+}\;
%			\delta_{cy}
%			\cdot
%			\mu_{1 \vert xy}
%		\;\right)\,,
%		\quad
%		\textnormal{by \,\eqref{MzeroImplies}, \,\eqref{MoneImpliesCEqualsY}, and definition of \,$\mu_{m \vert xy}$}
	\end{eqnarray*}

\end{frame}
\normalsize

%%%%%%%%%%

\begin{frame}{\vskip -0.20cm\Large Proof ...}

\tiny

	\begin{eqnarray*}
	&&
		E\!\left[\;
			\left.
			W^{(i)}_{c \vert xy{\color{red}0}}
			\,\;\right\vert
			\EMConditionsWithValues
		\right]
	\\
	&=&
		\overset{{\color{white}1}}{\cdots}
%	\\
%	&=&
%		I^{(i)}_{xy0}
%		\cdot
%		P\!\left(
%			\left.
%			Y^{(i)} = c
%			\,\;\right\vert
%			\!\!
%			\begin{array}{c}
%				X^{(i)} = x,\, \widetilde{Y}^{(i)} = y,\, J^{(i)} = 0
%			\end{array}
%			\textnormal{\large;}
%			\modelParameters
%		\!\!\right)
	\\
	&=&
		I^{(i)}_{xy0}
		\cdot
		P\!\left(
			\left.
			Y^{(i)} = c
			\,\;\right\vert
			\!\!
			\begin{array}{c}
				X^{(i)} = x,\, \widetilde{Y}^{(i)} = y
			\end{array}
			\textnormal{\large;}
			\;\;\cdots\;\;
		\right)\,,
		\quad
		\textnormal{by \eqref{ZJindependence} and suppressing parameters for brevity}
	\\
	&=&
		I^{(i)}_{xy0}
		\cdot
		\left\{\;
			P\!\left(\,
				\left.
				Y^{(i)} = c,\,M^{(i)}=0
				\;\right\vert
				X^{(i)} = x,\, \widetilde{Y}^{(i)} = y
			\;\right)
			\;+\;
			P\!\left(\,
				\left.
				Y^{(i)} = c,\,M^{(i)}=1
				\;\right\vert
				X^{(i)} = x,\, \widetilde{Y}^{(i)} = y
			\;\right)
		\;\right\}
	\\
	&=&
		I^{(i)}_{xy0}
		\cdot
		\left\{\;
		\begin{array}{cc}
			&
			P\!\left(\,
				\left.
				Y^{(i)} = c
				\;\right\vert
				M^{(i)}=0,\,X^{(i)} = x,\, \widetilde{Y}^{(i)} = y
			\;\right)
			\cdot
			P\!\left(\,
				\left.
				M^{(i)}=0
				\;\right\vert
				X^{(i)} = x,\, \widetilde{Y}^{(i)} = y
			\;\right)
		\\
			\overset{\textnormal{\large{\color{white}1}}}{+}&
			P\!\left(\,
				\left.
				Y^{(i)} = c
				\;\right\vert
				M^{(i)}=1,\, X^{(i)} = x,\, \widetilde{Y}^{(i)} = y
			\;\right)
			\cdot
			P\!\left(\,
				\left.
				M^{(i)}=1
				\;\right\vert
				X^{(i)} = x,\, \widetilde{Y}^{(i)} = y
			\;\right)
		\end{array}
		\;\right\}
	\\
	&=&
		I^{(i)}_{xy0}
		\cdot
		\left(\;
			\pi_{c \vert xy}
			\cdot
			\mu_{0 \vert xy}
			\;\overset{{\color{white}.}}{+}\;
			\delta_{cy}
			\cdot
			\mu_{1 \vert xy}
		\;\right)\,,
		\quad
		\textnormal{by \,\eqref{MzeroImplies}, \,\eqref{MoneImpliesCEqualsY}, and definition of \,$\mu_{m \vert xy}$}
	\end{eqnarray*}

\end{frame}
\normalsize

%%%%%%%%%%
