
\noindent
\textbf{Exercise 4.13(a)}

\vskip 0.3cm
\noindent
The likelihood function is:
\begin{equation*}
L(\theta)
\;=\;\prod_{i=1}^{n}\,f_{T}(t_{i};\theta)
\;=\;\prod_{i=1}^{n}\,\theta\,e^{-\theta\,t_{i}}
\;=\;\theta^{n}\,e^{-\,\theta\sum_{i=1}^{n}t_{i}}
\end{equation*}
The log likelihood function is:
\begin{equation*}
l(\theta)
\;=\; \log L(\theta)
\;=\; n\,\log(\theta) - \theta\,\sum_{i=1}^{n}\,t_{i}
\end{equation*}
\begin{equation*}
\dfrac{\partial l}{\partial\theta}
\;=\; \dfrac{n}{\theta} \, - \, \sum_{i=1}^{n}\,t_{i}
\end{equation*}
Thus,
\begin{equation*}
\dfrac{\partial l}{\partial\theta} \; = \; 0
\quad\Longrightarrow\quad
\theta \; = \; \dfrac{n}{\sum_{i=1}^{n}\,t_{i}}
\end{equation*}
Hence,
\begin{equation*}
\widehat{\theta}_{\textnormal{MLE}} \; = \; \dfrac{n}{\sum_{i=1}^{n}\,T_{i}}
\end{equation*}
Next, note that:
\begin{equation*}
\dfrac{\partial^{2}l}{\partial\theta^{2}}
\;=\; -\,\dfrac{n}{\theta^{2}}
\end{equation*}
Hence,
\begin{equation*}
n\,\textnormal{Var}\!\left[\widehat{\theta}_{\textnormal{MLE}}\right]
\;\approx\; n\left(-E\!\left[\dfrac{\partial^{2}l}{\partial\theta^{2}}\right]\right)^{-1}
\;=\; n\left(-E\!\left[-\,\dfrac{n}{\theta^{2}}\right]\right)^{-1}
\quad\Longrightarrow\quad
\textnormal{Var}\!\left[\widehat{\theta}_{\textnormal{MLE}}\right]
\;=\; \dfrac{\theta^{2}}{n}
\end{equation*}

%%%%%%%%%%%%%%%%%%%%%%%%%%%%%%%%%%%%%%%%%%%%%%%%%%%%%%%%%%%%%%%
\vskip 1.0cm
\noindent
\textbf{Exercise 4.13(b)}

\vskip 0.3cm
\noindent
First, note that
\begin{equation*}
P\!\left(Y=1\right)
\;=\; P\!\left(T > t^{*} \right)
\;=\; \int_{t^{*}}^{\infty}f_{T}(t;\theta)\,\dd t
\;=\; \int_{t^{*}}^{\infty}\theta\,e^{-\theta t}\,\dd t
\;=\; \theta\left[\,-\,\dfrac{e^{-\theta t}}{\theta}\,\right]_{t^{*}}^{\infty}
\;=\; e^{-\theta t^{*}}
\end{equation*}
Hence,
\begin{equation*}
P\!\left(Y=0\right)
\;=\; 1 - P\!\left(Y=1\right)
\;=\; 1 - e^{-\theta t^{*}}
\end{equation*}
The likelihood function is thus:
\begin{equation*}
L^{*}(\theta)
\;=\; \prod_{i=1}^{n}\,P(Y_{i}=1)^{Y_{i}}\,P(Y_{i}=0)^{1-Y_{i}}
\;=\; P(Y=1)^{\sum_{i=1}^{n}Y_{i}} \cdot P(Y=0)^{n - \sum_{i=1}^{n}Y_{i}}
\;=\; \left(e^{-\theta t^{*}}\right)^{S} \cdot \left(1-e^{-\theta t^{*}}\right)^{n - S}\,,
\end{equation*}
where $S := \sum_{i=1}^{n}Y_{i}$.
Hence, the log likelihood function is:
\begin{equation*}
l^{*}(\theta)
\;=\; \log L^{*}(\theta)
\;=\; -\,\theta t^{*}S \, + \, (n - S)\log\left(1 - e^{-\theta t^{*}}\right)
\end{equation*}
Hence,
\begin{equation*}
\dfrac{\partial l^{*}}{\partial\theta}
\;=\; -t^{*}S + \dfrac{n-S}{1-e^{-\theta t^{*}}}\left(-\,e^{-\theta t^{*}}\cdot(-t^{*})\right)
\;=\; -t^{*}S + \dfrac{t^{*}e^{-\theta t^{*}}(n-S)}{1 - e^{-\theta t^{*}}}
\end{equation*}
And,
\begin{equation*}
\dfrac{\partial l^{*}}{\partial\theta} \; = \; 0
\quad\Longrightarrow\quad\cdots\quad\Longrightarrow\quad
\widehat{\theta}^{*}
\;=\; \dfrac{1}{t^{*}}\log\left(\dfrac{n}{S}\right)
\;=\; \dfrac{1}{t^{*}}\log\left(\dfrac{n}{\sum_{i=1}^{n}Y_{i}}\right)
\end{equation*}

%%%%%%%%%%%%%%%%%%%%%%%%%%%%%%%%%%%%%%%%%%%%%%%%%%%%%%%%%%%%%%%
\vskip 1.0cm
\noindent
\textbf{Exercise 4.13(c)}

\begin{equation*}
\dfrac{\partial l^{*}}{\partial\theta}
\;=\; -t^{*}S + \dfrac{t^{*}e^{-\theta t^{*}}(n-S)}{1 - e^{-\theta t^{*}}}
\;=\; -t^{*}S + (n-S)\cdot t^{*}\cdot e^{-\theta t^{*}}\cdot\left(1 - e^{-\theta t^{*}}\right)^{-1}
\end{equation*}
And,
\begin{equation*}
\dfrac{\partial^{2}l^{*}}{\partial\theta^{2}}
\;=\;\cdots\;=\;
\;=\; -\,(n-S)\,\dfrac{e^{-\theta t^{*}}(t^{*})^{2}}{\left(1 - e^{-\theta t^{*}}\right)^{2}}
\end{equation*}
Now, note that:\;\;$S \; \sim \; \textnormal{Binomial}\!\left(\,n,\,e^{-\theta t^{*}}\,\right)$.
Hence,
\begin{equation*}
E\!\left[\,\dfrac{\partial^{2}l^{*}}{\partial\theta^{2}}\,\right]
\;=\; -\,(n-E[\,S\,])\,\dfrac{e^{-\theta t^{*}}(t^{*})^{2}}{\left(1 - e^{-\theta t^{*}}\right)^{2}}
\;=\; -\,(n-n\,e^{-\theta t^{*}})\,\dfrac{e^{-\theta t^{*}}(t^{*})^{2}}{\left(1 - e^{-\theta t^{*}}\right)^{2}}
\;=\; \dfrac{n\,e^{-\theta t^{*}}(t^{*})^{2}}{\left(e^{-\theta t^{*}} - 1\right)}
\;=\; \dfrac{n(t^{*})^{2}}{\left(1 - e^{{\color{red}+}\theta t^{*}}\right)}
\end{equation*}
Hence,
\begin{equation*}
\textnormal{Var}\!\left[\,\widehat{\theta}^{*}\,\right]
\;=\; -\,\left(E\!\left[\,\dfrac{\partial^{2}l^{*}}{\partial\theta^{2}}\,\right]\right)^{-1}
\;=\; \dfrac{\left(e^{\theta t^{*}} - 1\right)}{n(t^{*})^{2}}
\end{equation*}
Thus,
\begin{equation*}
\dfrac{\textnormal{Var}\!\left[\,\widehat{\theta}_{\textnormal{MLE}}\,\right]}{\textnormal{Var}\!\left[\,\widehat{\theta}^{*}\,\right]}
\;=\; \dfrac{\theta^{2}}{n}\cdot\dfrac{n(t^{*})^{2}}{\left(e^{\theta t^{*}} - 1\right)}
\;=\; \dfrac{(\theta t^{*})^{2}}{\left(e^{\theta t^{*}} - 1\right)}
\end{equation*}







