
          %%%%% ~~~~~~~~~~~~~~~~~~~~ %%%%%

\section{Etemadi's inequality}
\setcounter{theorem}{0}
\setcounter{equation}{0}

\renewcommand{\theenumi}{\roman{enumi}}
\renewcommand{\labelenumi}{\textnormal{(\theenumi)}$\;\;$}

\begin{theorem}[Appendix M19, \cite{Billingsley1999}]
\label{EtemadiInequality}
\mbox{}\vskip 0.1cm
\noindent
Suppose $X_{1}, \ldots , X_{n} : \Omega \longrightarrow \Re$ are independent
$\Re$-valued random variables defined on the common probability space $\Omega$.
Let $S_{k} \,:=\, \overset{k}{\underset{i=1}{\textnormal{\large$\sum$}}}\,X_{i}$, for $k = 1, 2, \ldots, n$.
Then, for any $x > 0$,
\begin{equation*}
P\!\left(\left\{\;
	\omega \in \Omega
	\;\left\vert\;
	\underset{1\leq k \leq n}{\max}\,\vert\,S_{k}(\omega)\,\vert \,\overset{{\color{white}:}}{\geq}\, 3x
	\right.
\;\right\}\right)
\;\; \leq \;\;
3 \cdot \underset{1\leq k \leq n}{\max}\;
P\!\left(\left\{\;
	\omega \in \Omega
	\;\left\vert\;\,
	\vert\,S_{k}(\omega)\,\vert \,\overset{{\color{white}1}}{\geq}\, x
	\right.
\;\right\}\right).
\end{equation*}
\end{theorem}
\proof
Define:
\begin{eqnarray*}
A_{{\color{white}0}} & := &
\left\{\;
	\omega \in \Omega
	\;\left\vert\;\,
	\underset{1\leq k \leq n}{\max}\,\vert\,S_{k}(\omega)\,\vert \,\overset{{\color{white}:}}{\geq}\, 3x
	\right.
\;\right\},
\\
A_{1} & := &
\left\{\;
	\omega \in \Omega
	\;\left\vert\;\,
	\vert\,S_{1}(\omega)\,\vert \overset{{\color{white}:}}{\geq} 3x
	\right.
\;\right\},
\\
A_{k} & := &
\left\{\;
	\omega \in \Omega
	\;\left\vert\;\,
	\underset{1\leq i \leq k-1}{\max}\,\vert\,S_{i}(\omega)\,\vert \overset{{\color{white}:}}{<} 3x
	\;\;\textnormal{and}\;\;
	\vert\,S_{k}(\omega)\,\vert\,\geq\,3x
	\right.
\;\right\},
\quad\textnormal{for $k = 2, 3, \ldots, n$}.
\end{eqnarray*}
Note that $A$ can be expressed as the following disjoint union:\;
$A \; = \; \overset{n}{\underset{k=1}{\bigsqcup}}\;A_{k}$.

\vskip 0.5cm
\begin{center}
\begin{minipage}{6.5in}
\noindent
\textbf{Claim 1:}\quad
$A_{k}\overset{{\color{white}:}}{\cap}\left\{\,\vert\,S_{n}\,\vert \overset{{\color{white}.}}{<} x\,\right\}
\,\subset\,
A_{k}\overset{{\color{white}:}}{\cap}\left\{\,\vert\,S_{n}-S_{k}\,\vert \overset{{\color{white}.}}{>} 2x\,\right\}$,\;
for each $k = 1, 2, \ldots, n$.

\vskip 0.3cm
\noindent
\textbf{Claim 2:}\quad
$\left\{\,\vert\,S_{n} - S_{k}\,\vert \overset{{\color{white}.}}{>} 2x\,\right\}
\;\subset\;
\left\{\,\vert\,S_{n}\,\vert \overset{{\color{white}.}}{>} x\,\right\}
\,\bigcup\,
\left\{\,\vert\,S_{k}\,\vert \overset{{\color{white}.}}{>} x\,\right\}$,\;
for each $k = 1, 2, \ldots, n$.
\end{minipage}
\end{center}

\vskip 0.5cm
\noindent
Proof of Claim 1:\quad
\begin{eqnarray*}
&&
	\omega \in A_{k}\overset{{\color{white}:}}{\cap}\left\{\,\vert\,S_{n}\,\vert \overset{{\color{white}.}}{<} x\,\right\}
\\
&\Longleftrightarrow&
	\underset{1\leq i \leq k-1}{\max} \left\vert\,S_{i}(\overset{{\color{white}.}}{\omega})\,\right\vert< 3x
	\;\;\textnormal{and}\;\;
	\left\vert\,S_{k}(\overset{{\color{white}.}}{\omega})\,\right\vert\,\geq\,3x
	\;\;\textnormal{and}\;\;
	\left\vert\,S_{n}(\overset{{\color{white}.}}{\omega})\,\right\vert\,<\,x
\\
&\Longrightarrow&
	\underset{1\leq i \leq k-1}{\max} \left\vert\,S_{i}(\overset{{\color{white}.}}{\omega})\,\right\vert< 3x
	\;\;\textnormal{and}\;\;
	\left\vert\,S_{k}(\overset{{\color{white}.}}{\omega})\,\right\vert\,\geq\,3x
	\;\;\textnormal{and}\;\;
	\left\vert\;S_{k}(\omega) \overset{{\color{white}.}}{-} S_{n}(\omega)\;\right\vert
	\;\geq\; \left\vert\,S_{k}(\overset{{\color{white}.}}{\omega})\,\right\vert \,-\, \left\vert\,S_{n}(\overset{{\color{white}.}}{\omega})\,\right\vert
	\;>\; 3x - x \; = \; 2x
\\
&\Longrightarrow&
	\omega \in A_{k}\overset{{\color{white}:}}{\cap}\left\{\,\vert\,S_{n}-S_{k}\,\vert \overset{{\color{white}.}}{>} 2x\,\right\}
\end{eqnarray*}
This proves Claim 1.

\vskip 0.8cm
\noindent
Proof of Claim 2:\quad
Simply note that for any two real numbers $a, b \in \Re$, we have:
\begin{equation*}
\vert\,a\,\vert \;\leq\; x
\;\;\textnormal{and}\;\;
\vert\,b\,\vert \;\leq\; x
\quad\Longrightarrow\quad
\vert\,a - b\,\vert \;\leq\; \vert\,a\,\vert \;+\; \vert\,b\,\vert \;\leq\; x \;+\; x \;=\; 2x,
\end{equation*}
whose contrapositive is:
\begin{equation*}
\vert\,a - b\,\vert \;>\; 2x,
\quad\Longrightarrow\quad
\vert\,a\,\vert \;>\; x
\;\;\textnormal{or}\;\;
\vert\,b\,\vert \;>\; x.
\end{equation*}
This proves Claim 2.

\vskip 0.8cm
\noindent
Using the above two Claims, we now see that:
\begin{eqnarray*}
P(A)
&=&
	P\!\left(\,A\overset{{\color{white}.}}{\cap}\{\,\vert\,S_{n}\,\vert\geq x\,\}\,\right)
	\;+\; P\!\left(\,A\overset{{\color{white}.}}{\cap}\{\,\vert\,S_{n}\,\vert < x\,\}\,\right)
\\
&\leq&
	P\!\left(\,\vert\,S_{n}\,\vert \overset{{\color{white}.}}{\geq} x\,\right)
	\;+\; P\!\left(\,A\overset{{\color{white}:}}{\cap}\{\,\vert\,S_{n}\,\vert < x\,\}\,\right)
\\
&=&
	P\!\left(\,\vert\,S_{n}\,\vert \overset{{\color{white}.}}{\geq} x\,\right)
	\;+\; \overset{n}{\underset{k=1}{\sum}}\; P\!\left(\,A_{k}\overset{{\color{white}:}}{\cap}\{\,\vert\,S_{n}\,\vert < x\,\}\,\right)
\\
&\leq&
	P\!\left(\,\vert\,S_{n}\,\vert \overset{{\color{white}.}}{\geq} x\,\right)
	\;+\; \overset{n}{\underset{k=1}{\sum}}\; P\!\left(\,A_{k}\overset{{\color{white}:}}{\cap}\{\,\vert\,S_{n}-S_{k}\,\vert > 2x\,\}\,\right),
	\quad\quad\textnormal{by Claim 1}
\\
&=&
	P\!\left(\,\vert\,S_{n}\,\vert \overset{{\color{white}.}}{\geq} x\,\right)
	\;+\;
		\overset{n}{\underset{k=1}{\sum}}\;
		P\!\left(\,A_{k}\,\right)\cdot P\!\left(\;\vert\,S_{n}-S_{k}\,\vert \overset{{\color{white}.}}{>} 2x\;\right),
	\quad\quad\textnormal{by independence of summands}
\\
&\leq&
	P\!\left(\,\vert\,S_{n}\,\vert \overset{{\color{white}.}}{\geq} x\,\right)
	\;+\;
		\left(\underset{1\leq k \leq n}{\max}\;P\!\left(\,\vert\,S_{n}-S_{k}\,\vert \overset{{\color{white}.}}{>} 2x\,\right)\right)
		\cdot
		\overset{n}{\underset{k=1}{\sum}}\; P\!\left(\,A_{k}\,\right)
\\
&=&
	P\!\left(\,\vert\,S_{n}\,\vert \overset{{\color{white}.}}{\geq} x\,\right)
	\;+\;
		P\!\left(\,A\,\right) \cdot
		\underset{1\leq k \leq n}{\max}\;P\!\left(\,\vert\,S_{n}-S_{k}\,\vert \overset{{\color{white}.}}{>} 2x\,\right)
\\
&=&
	P\!\left(\,\vert\,S_{n}\,\vert \overset{{\color{white}.}}{\geq} x\,\right)
	\;+\; \underset{1\leq k \leq n}{\max}\;P\!\left(\,\vert\,S_{n}-S_{k}\,\vert \overset{{\color{white}.}}{>} 2x\,\right)
\\
&\leq&
	P\!\left(\,\vert\,S_{n}\,\vert \overset{{\color{white}.}}{\geq} x\,\right)
	\;+\;
	\underset{1\leq k \leq n}{\max}\;\left\{\;
		P\!\left(\,\vert\,S_{n}\,\vert \overset{{\color{white}.}}{>} x\,\right)
		\;+\;
		P\!\left(\,\vert\,S_{k}\,\vert \overset{{\color{white}.}}{>} x\,\right)
	\;\right\},
	\quad\quad\textnormal{by Claim 2}
\\
&\leq&
	3\,\cdot\,\underset{1\leq k \leq n}{\max}\left\{\;
		P\!\left(\,\vert\,S_{k}\,\vert \overset{{\color{white}.}}{\geq} x\,\right)
	\;\right\}.
\end{eqnarray*}
This completes the proof of Etemadi's inequality.
\qed

          %%%%% ~~~~~~~~~~~~~~~~~~~~ %%%%%
